<section xml:id="sec_Rings_ExtensionRings">
  <title>Extension Rings</title>
  <p>
    We have learned that a subring can be formed from a subset of a ring.
    One example we used was that
    <m>\{0,2,4\}</m> is a subring of <m>{\mathbb Z}_6</m>.
    We can also extend a ring into a larger set, called an extension ring.
    We would say that <m>{\mathbb Z}_6</m> is an extension ring of <m>\{0,2,4\}</m>.
  </p>
  <definition>
    <statement>
      <p>
        {ext_ring} If <m>R</m> is a subring of <m>S</m>,
        then we can say that <m>S</m> is an
        <term>extension ring</term> of <m>R</m>.
      </p>
    </statement>
  </definition>
  <p>
    Extension rings can be used to create number systems that are more "complete" in some sense.
    In fact, you've seen extension rings several times before.
    The integers form a very simple number system,
    but integers lack multiplicative inverses.
    The set of rational numbers is in fact an extension ring of the integers,
    which includes the multiplicative inverses that integers lack.
    Similarly, real numbers are "incomplete" in the sense that some real numbers do not have roots (e.g. there is no real square root of -1).
    The complex numbers form a larger number system that includes the real numbers,
    and also has the missing roots.
  </p>
  <p>
    Another example of extension ring that we've seen before is the polynomial ring <m>{\mathbb Q}[x]</m>,
    which contains the ring <m>{\mathbb Q}</m>.
    Some polynomials lack multiplicative inverses as the following proposition shows.
  </p>
  <proposition>
    <statement>
      <p>
        <m>p(x)=1+x</m> has no multiplicative inverse in <m>{\mathbb Q}[x]</m>.
      </p>
    </statement>
    <proof>
      <p>
        We will show by contradiction that <m>1 + x</m> has no multiplicative inverse in <m>{\mathbb Q}[x]</m>.
        Suppose on the contrary that <m>1+x</m> has an inverse that can be written as <m>q(x) = \sum_{n=0}^{N}a_nx^n</m>,
        where <m>a_N</m> is the leading nonzero coefficient and <m>N \ge 0</m>.
        Then
        <me>
          (1+x)q(x) = (1+x) \cdot \sum_{n=0}^{N}a_nx^n=a_{N}x^{N+1}+\cdots+a_0
        </me>.
      </p>
      <p>
        Since <m>a_N \neq 0</m>,
        it follows that the degree of
        <m>(1+x)q(x)</m> is equal to <m>N+1</m>,
        so it is not a constant polynomial.
        In particular, <m>(1+x)q(x) \neq 1</m>.
        This contradicts the supposition that <m>q(x)</m> is the multiplicative inverse of <m>1+x</m>.
        Therefore, <m>(1+x)</m> does not have a multiplicative inverse in <m>{\mathbb Q}[x]</m>.
      </p>
    </proof>
  </proposition>
  <p>
    We can actually go further,
    and take infinite power series in addition to finite polynomials.
    This gives us an even larger extension ring:
  </p>
  <p>
    Let <m>\widehat{{\mathbb Q}}[x]</m> be the set of power series with rational coefficients:
    <md>
      <mrow>\widehat{{\mathbb Q}}[x]=\{\sum_{n=0}^{\infty}a_n x^n\}~\text{ , where } ~a_n\in {\mathbb Q}.</mrow>
      <mrow>\text{ Show that } ~ \widehat{{\mathbb Q}}[x]~\text{ is an extension ring of } ~{\mathbb Q}[x]</mrow>
    </md>.
  </p>
  <p>
    Now, the question is does <m>p(x)</m> have a multiplicative inverse in <m>\widehat{{\mathbb Q}}[x]</m>?
    There are 3 methods we can do to figure this out.
    <ol>
      <li>
        <p>
          Taylor series
        </p>
      </li>
      <li>
        <p>
          Long division
        </p>
      </li>
      <li>
        <p>
          Linear recurrence relation
        </p>
      </li>
    </ol>
  </p>
  <p>
    We will explore all three methods in the following example.
  </p>
  <example xml:id="example_Rings_Zx">
    <statement>
      Find the multiplicative inverse of <m>(1+x)</m> in <m>\widehat{{\mathbb Z}}[x]</m>
      <ol>
        <li>
          <p>
            First Method: Taylor series  The Taylor series expansion for the function <m>f(x)</m> about the point <m>a=0</m> is given by:
            <me>
              f(x)=f(0)+f'(0)x+\frac{f''(0)x^2}{2!}+\frac{f'''(0)x^3}{3!}+\cdots
            </me>
            For <m>f(x)=\frac{1}{1+x}</m> , we have:
            <md>
              <mrow>\left(\frac{1}{1+x}\right)'\amp =((1+x)^{-1})'=-1!(1+x)^{-2}\implies \text{ when \(x=0,~f'(x)=-1\) }</mrow>
              <mrow>((1+x)^{-1})''\amp =-1(-2)(1+x)^{-3}=2!(1+x)^{-3}\implies \text{ when \(x=0,~f''(x)=2\) }</mrow>
              <mrow>((1+x)^{-1})'''\amp =2(-3)(1+x)^{-4}=-3!(1+x)^{-4} \implies \text{ when \(x=0,~f'''(x)=-3\) }</mrow>
              <mrow>\text{ In general: }</mrow>
              <mrow>((1+x)^{-1})^{(n)}\amp =(-1)^{n}n!(1+x)^{-n-1} \implies \text{when \(x=0,~f^n(x)=(-1)^{n}n!\)}</mrow>
            </md>
            Therefore,
            <men>
              (1+x)^{-1}=1-x+x^2-x^3+\cdots=\sum_{n=0}^{\infty}(-1)^nx^n\in \widehat{{\mathbb Q}}[x]
            </men>
            This is a multiplicative inverse of <m>(1+x)</m> in <m>\widehat{{\mathbb Z}}[x]</m>
            (also in <m>\widehat{{\mathbb Q}}[x]</m>).
          </p>
        </li>
        <li>
          <p>
            Second Method: Long Division Use long division to divide <m>\frac{1}{1+x}:</m>
            <tabular>
              <row>
                <cell></cell>
                <cell><m>1</m></cell>
                <cell><m>-</m></cell>
                <cell><m>x</m></cell>
                <cell><m>+</m></cell>
                <cell><m>x^2</m></cell>
                <cell><m>-</m></cell>
                <cell><m>x^3</m></cell>
                <cell><m>+</m></cell>
                <cell><m>\cdots</m></cell>
              </row>
              <row>
                <cell><m>1 + x</m></cell>
                <cell><m>1</m></cell>
                <cell><m>+</m></cell>
                <cell><m>0x</m></cell>
                <cell><m>+</m></cell>
                <cell><m>0x^2</m></cell>
                <cell><m>+</m></cell>
                <cell><m>0x^3</m></cell>
                <cell><m>+</m></cell>
                <cell><m>\cdots</m></cell>
              </row>
              <row>
                <cell></cell>
                <cell><m>-1</m></cell>
                <cell><m>+</m></cell>
                <cell><m>-x</m></cell>
              </row>
              <row>
                <cell></cell>
                <cell></cell>
                <cell></cell>
                <cell><m>-x</m></cell>
                <cell><m>+</m></cell>
                <cell><m>0x^2</m></cell>
              </row>
              <row>
                <cell></cell>
                <cell></cell>
                <cell></cell>
                <cell><m>+x</m></cell>
                <cell><m>+</m></cell>
                <cell><m>x^2</m></cell>
              </row>
              <row>
                <cell></cell>
                <cell></cell>
                <cell></cell>
                <cell></cell>
                <cell></cell>
                <cell><m>x^2</m></cell>
                <cell><m>+</m></cell>
                <cell><m>0x^3</m></cell>
              </row>
              <row>
                <cell></cell>
                <cell></cell>
                <cell></cell>
                <cell></cell>
                <cell></cell>
                <cell><m>-x^2</m></cell>
                <cell><m>-</m></cell>
                <cell><m>x^3</m></cell>
              </row>
              <row>
                <cell></cell>
                <cell></cell>
                <cell></cell>
                <cell></cell>
                <cell></cell>
                <cell></cell>
                <cell></cell>
                <cell><m>-x^3</m></cell>
                <cell><m>+</m></cell>
                <cell><m>\cdots</m></cell>
              </row>
              <row>
                <cell></cell>
                <cell></cell>
                <cell></cell>
                <cell></cell>
                <cell></cell>
                <cell></cell>
                <cell></cell>
                <cell></cell>
                <cell><m>\vdots</m></cell>
              </row>
            </tabular>
          </p>
        </li>
        <li>
          <p>
            Third Method: Linear Recurrence Relation:   We want:
            <me>
              1=(a+x)\sum_{n=0}^{\infty}a_nx^n=1+0x+0x^2+\cdots
            </me>
            Use distributive law:
            <md>
              <mrow>1\amp =a\sum_{n=0}^{\infty}a_nx^n+x\sum_{n=0}^{\infty}a_nx^{n}  \amp  \text{ distributive law }</mrow>
              <mrow>\amp =\sum_{n=0}^{\infty}a_nx^n+\sum_{n=0}^{\infty}a_nx^{n+1} \amp  \text{ simplify }</mrow>
              <mrow>\amp =\sum_{n=0}^{\infty}a_nx^n+\sum_{n=1}^{\infty}a_{n-1}x^{n} \amp  \text{ change second summation index }</mrow>
              <mrow>\amp =a_0+\sum_{n=1}^{\infty}a_nx^n+\sum_{n=1}^{\infty}a_{n-1}x^{n} \amp  \text{ separate one term from sum }</mrow>
              <mrow>\amp =a_0+\sum_{n=1}^{\infty}(a_nx^n+a_{n-1}x^n) \amp  \text{ combine two sums }</mrow>
              <mrow>\amp =a_0+\sum_{n=1}^{\infty}(a_n+a_{n-1})x^n \amp  \text{ factor out \(x_n\) }</mrow>
            </md>
            Now we can write:
            <md>
              <mrow>1+0x+0x^2+\cdots=a_0+\sum_{n=1}^{\infty}(a_n+a_{n-1})x^n</mrow>
            </md>
            Equate like powers of <m>x</m> for the two polynomials:
            <md>
              <mrow>1\amp =a_0</mrow>
              <mrow>0\amp =a_1+a_0=a_1+1\implies a_1=-1</mrow>
              <mrow>0\amp =a_2+a_1=a_2+-1\implies a_2=1</mrow>
              <mrow>0\amp =a_3+a_2=a_3+1\implies a_3=-1</mrow>
              <mrow>0\amp =a_4+a_3=a_4+-1\implies a_4=1</mrow>
              <mrow>\vdots</mrow>
              <mrow>0\amp =a_n+a_{n-1}\implies a_n=(-1)^n</mrow>
            </md>
          </p>
        </li>
      </ol>
    </statement>
  </example>
  <exercise>
    <statement>
      <p>
        Find the inverse of <m>a+x</m> in <m>\widehat{{\mathbb Q}}[x]</m> by the:
        <ol>
          <li>
            <p>
              long division method
            </p>
          </li>
          <li>
            <p>
              recurrence relation method
            </p>
          </li>
        </ol>
      </p>
    </statement>
  </exercise>
  <exercise xml:id="exercise_Rings_Z2x">
    <statement>
      <p>
        Find the inverse of <m>1+x</m> in <m>\widehat{{\mathbb Z}}_{2}[x]</m> by the:
        <ol type="a">
          <li>
            <p>
              long division method
            </p>
          </li>
          <li>
            <p>
              recurrence relation method
            </p>
          </li>
        </ol>
      </p>
    </statement>
  </exercise>
  <exercise>
    <statement>
      <p>
        Find the inverse of <m>3+2x</m> in <m>\widehat{{\mathbb Z}}_{5}[x]</m> by the:
        <ol type="a">
          <li>
            <p>
              long division method
            </p>
          </li>
          <li>
            <p>
              recurrence relation method
            </p>
          </li>
        </ol>
      </p>
    </statement>
  </exercise>
  <exercise xml:id="exercise_Rings_Z5x">
    <statement>
      <p>
        Find the multiplicative inverse of
        <m>(1+2x+3x^2)</m> in <m>\widehat{{\mathbb Z}}_5[x]</m>,
        in <m>\widehat{{\mathbb Z}}_7[x]</m>,
        and in <m>\widehat{{\mathbb Q}}[x]</m> by the:
        <ol type="a">
          <li>
            <p>
              long division method
            </p>
          </li>
          <li>
            <p>
              recurrence relation method
            </p>
          </li>
        </ol>
      </p>
    </statement>
  </exercise>
</section>