<section xml:id="sec_SigmaNotation_SumByParts">
  <title>Summation by parts</title>
  <p>
    Those who have studied integrals in calculus may be familiar with the process of integration by parts.
    This is used when you need to find the integral of the product of two terms.
    While this process is used for continuous situations,
    there is a version of this process for discrete situations called
    <term>summation by parts</term>.
  </p>
  <p>
    To show how summation by parts works,
    we'll look at a particular case.
    Consider the following product of sums:
    <me>
      \left( \sum_{n=1}^{5}a_{n} \right) \left( \sum_{n=1}^{5}b_{n} \right)
    </me>.
  </p>
  <p>
    If we broke this up into individual terms,
    we'd obtain <m>n \cdot n = n^2</m> terms of the form <m>a_j b_k</m>.
    <xref ref="fig_IBP">Figure</xref>
    shows the terms arranged on a grid.
    We've separated these terms into two parts using a diagonal line,
    and we've further grouped terms either by row
    (above the line)
    or by column
    (below the line).
    You'll see in a minute why we've arranged things like this.
  </p>
  <figure xml:id="fig_IBP">
    <caption>Arrangements of terms in the product of sums <m>\left( \sum_{n=1}^{5}a_{n} \right) \left( \sum_{n=1}^{5}b_{n} \right)</m>.</caption>
    <image width="56%" source="images/IBP.png"/>
  </figure>
  <p>
    Now let's go back and express the sum of all these terms a different way.
    We'll introduce the notation:
    <me>
      A_{k}= \sum_{j=1}^{k}a_{j} \text{ and }  B_{k}= \sum_{j=1}^{k}b_{j}
    </me>.
  </p>
  <p>
    <m>A_k</m> and <m>B_k</m> are the <m>k</m>th <term>partial sums</term>
    for the series <m>\sum a_j</m> and <m>\sum b_j</m>, respectively.
    The product of sums that we started with can be written succinctly as <m>A_{5}B_{5}</m>.
  </p>
  <p>
    We may use this new notation to re-express the grouped terms in the figure.
    Consider first the terms below the diagonal line.
    These terms are grouped by column,
    and each group is encircled by an oval:
    <ul>
      <li>
        <p>
          The sum of the first oval(column on far left) is:
          <m>a_{1}b_{1}= a_{1}B_{1}</m>;
        </p>
      </li>
      <li>
        <p>
          The sum of the second oval(column second from the left) is:
          <m>a_{2}\left ( b_{1}+b_{2} \right )= a_{2}B_{2}</m>;
        </p>
      </li>
      <li>
        <p>
          The sum the third oval(column third from the left) is:
          <m>a_{3}\left ( b_{1}+b_{2}+b_{3} \right )= a_{3}B_{3}</m>;
        </p>
      </li>
      <li>
        <p>
          The sum of the fourth oval(column fourth from left) is:
          <m>a_{4}\left ( b_{1}+b_{2}+b_{3}+b_{4} \right )= a_{4}B_{4}</m>;
        </p>
      </li>
      <li>
        <p>
          The sum of the fifth oval(column on the far right) is:
          <m>a_{5}\left (b _{1}+b_{2}+b_{3}+b_{4}+b_{5} \right )=a _{5}B_{5}</m>.
        </p>
      </li>
    </ul>
  </p>
  <p>
    Adding these five sums together accounts for all the terms below the diagonal line:
    <me>
      a_1B_1 + a_2B_2 + \ldots + a_5B_5 = \sum_{k=1}^{5}a_kB_k
    </me>,
    where we've used summation notation to make the expression more compact.
  </p>
  <p>
    Now let's repeat this process for the horizontal ovals above the diagonal line:
    <ul>
      <li>
        <p>
          The sum for the first oval(bottom row above line) is:
          <m>a_{1}b_{2}= A_{1}b_{2}</m>;
        </p>
      </li>
      <li>
        <p>
          The sum for the second oval( second row from bottom) is:
          <m>\left ( a_{1}+a_{2} \right)b_{3}= A_{2}b_{3}</m>;
        </p>
      </li>
      <li>
        <p>
          The sum for the third oval(second row from the top) is:
          <m>\left ( a_{1}+a_{2}+a_{3} \right )b_{4}= A_{3}b_{4}</m>;
        </p>
      </li>
      <li>
        <p>
          The sum for the fourth oval(top row) is:
          <m>\left ( a_{1}+a_{2}+a_{3}+a_{4} \right)b_{5}= A_{4}b_{5}</m>.
        </p>
      </li>
    </ul>
  </p>
  <p>
    Adding these five sums together accounts for all the terms below the diagonal line:
    <me>
      A_1b_2 +  \ldots + A_4b_5 = \sum_{k=1}^{5-1}A_kb_{k+1}
    </me>.
  </p>
  <p>
    Since we've now accounted for terms both above and below the line,
    we obtain the sum of all terms by adding together:
    <me>
      A_{5}B_{5}= \sum_{k=1}^{5}a_{k}B_{k}+\sum_{k=1}^{5-1}A_{k}b_{k+1}
    </me>.
  </p>
  <p>
    By rearranging this equation, we find:
    <me>
      \sum_{k=1}^{5}a_{k}B_{k}= A_{5}B_{5}-\sum_{k=1}^{5-1}A_{k}b_{k+1}
    </me>.
  </p>
  <p>
    There's really nothing special about the number <sq>5</sq> in our above expression<ndash/>we just chose it because this was a relatively simple case that we could illustrate.
    To get the general formula, we simply replace '5' with '<m>n</m>':
    <me>
      \sum_{k=1}^{n}a_{k}B_{k}= A_{n}B_{n}-\sum_{k=1}^{n-1}A_{k}b_{k+1}
    </me>.
  </p>
  <p>
    Notice the striking similarity between this formula and the formula for integration by parts:
    <me>
      \int_a^b u dv =\left. uv\right|_a^b - \int_a^b v du
    </me>.
  </p>
  <p>
    The resemblance makes a lot of sense,
    since integration is essentially a kind of summation (more precisely,
    a summation taken to a limit.)
  </p>
  <p>
    Now let's look at some examples to see how we can make use of this formula.
  </p>
  <example>
    <statement>
      <p>
        Evaluate <m>\sum_{k=1}^{n}2^{k-1}k</m>.
      </p>
      <p>
        In order to use the summation by parts formula,
        we need to define <m>a_k</m> and <m>B_k</m> so that the summand
        <m>2^{k-1}k</m> is the product of <m>a_k</m> and <m>B_k</m>.
        Just as in integration by parts,
        we want to make our choice based on what makes the calculations easiest.
        Note that <m>B_{k}</m> is a partial sum of <m>k</m> terms,
        and that <m>k = 1 + \ldots + 1</m>.
        So it's natural to choose <m>B_{k}=k</m>,
        which means that <m>a_{k}=2^{k-1}</m>.
      </p>
      <p>
        Based on our choice of <m>B_{k}</m> and <m>a_{k}</m>,
        we can now figure out <m>b_{k}</m> and <m>A_{k}</m>.
        As we noted above,
        <m>B_{k}</m> is the sum of <m>k</m> 1's, so that <m>b_k=1</m>.
        This leaves us with <m>a_k = 2^{k-1}</m>, so that
        <me>
          A_{k}=\sum_{j=1}^{k}a_j
        </me>.
      </p>
      <p>
        As we've seen before,
        we may rewrite this by shifting the starting value of the index, so that
        <me>
          A_{k}=\sum_{j'=0}^{k-1}2^{j'} =  \frac{2^k-1}{2-1} = 2^k-1
        </me>,
        where we've used our standard formula for the sum of geometric series.
      </p>
      <p>
        Summarizing our progress so far, we have:
        <me>
          a_k=2^{k-1}; B_k=k;  b_k=1;  A_k=2^k-1
        </me>.
      </p>
      <p>
        Plugging the above values into the summation by parts formula, we find:
        <me>
          \sum_{k=1}^{n}2^{k-1}k= \left (2 ^{n}-1 \right )n-\sum_{k=1}^{n-1}\left ( 2^{k}-1 \right )
        </me>.
      </p>
      <p>
        The summation on the far right can be evaluated by breaking it into two separate parts:
        <me>
          \sum_{k=1}^{n-1}\left ( 2^{k}-1 \right )= \sum_{k=1}^{n-1}2^{k}-\sum_{k=1}^{n-1}1 = (2^{n}-1)- (n-1)
        </me>.
      </p>
    </statement>
  </example>
  <p>
    We can put this into our equality and do some further algebraic puttering to obtain the final result:
    <md>
      <mrow>\sum_{k=1}^{n}2^{k-1}k \amp = (2 ^{n}-1)n- (2^{n}-1)+(n-1)</mrow>
      <mrow>\amp =  2^{n}n-n-(2^{n}-1)+(n-1)</mrow>
      <mrow>\amp =  2^{n}n-2^{n}</mrow>
      <mrow>\amp =  2^{n}(n-1)</mrow>
    </md>.
  </p>
  <exercise>
    <statement>
      <p>
        Evaluate <m>\sum_{k=1}^{n}k^{2}</m> by taking <m>B_k=k</m> and <m>a_k = k</m>.
        You will need the expression for the sum
        <m>1 + 2 + \ldots + m</m> that we derived previously.
      </p>
    </statement>
  </exercise>
  <p>
    From the preceding examples we may see that <m>B_k = k</m> is a frequent choice.
    This is closely related to the fact that <m>u=x</m> is a frequent choice when applying the integration by parts formula.
  </p>
  <exercise>
    <statement>
      <p>
        Prove the following equation using summation by parts:
        <me>
          \sum_{k=1}^n k^3 = \frac{n^4}{4} + \frac{n^3}{2} + \frac{n^2}{4}
        </me>
      </p>
    </statement>
  </exercise>
  <exercise>
    <statement>
      <ol type="a">
        <li>
          <p>
            Evaluate <m>\sum_{k=1}^{n}3^{k}k</m>.
          </p>
        </li>
        <li>
          <p>
            Evaluate <m>\sum_{k=1}^{n}3^{k}k^2</m>.
          </p>
        </li>
        <li>
          <p>
            Evaluate <m>\sum_{k=1}^{7n} \cis(2\pi k/7)\cdot k</m>.
          </p>
        </li>
      </ol>
    </statement>
  </exercise>
</section>