<section xml:id="sec_SigmaNotation_Hints">
  <title>Hints for
  <q>Sigma Notation</q>
  and
  <q>Applications of Sigma Notation</q>
  exercises</title>
  <p>
    <xref ref="exercise_SigmaNotation_nested2">Exercise</xref>(e): This is a more difficult one.
    Exchange order of summation.
    You will need to use a summation formula from the next section.
    The denominator factors as the difference of squares.
    Part of the final answer will look like <m>1 + 1/2 + 1/3 + \ldots + 1/19</m>,
    which you can evaluate using a spreadsheet or some other method.
  </p>
  <p>
    <xref ref="exercise_SigmaApp_detId">Exercise</xref>: Both sides are 0 if any of the two indices <m>i,j,k</m> are equal
    (show this).
    Then you only need to consider the three possible cases where <m>i,j,k</m> are all unequal.
  </p>
  <p>
    <xref ref="exercise_SigmaApp_nonzeroVec">Exercise</xref>(a): You will need to change around the indices in the formula from <xref ref="exercise_SigmaApp_2epsIdent">Exercise</xref>.
    Make the following replacements:
    <m>k \rightarrow i, i \rightarrow j, j \rightarrow k</m>.
    Then use the fact that <m>\epsilon_{ijk}= \epsilon_{jki}</m> (see <xref ref="exercise_SigmaApp_KLC">Exercise</xref>. to obtain
    <me>
      \sum_i \epsilon_{ijk} \epsilon_{imn} = \delta_{jm} \delta_{kn} - \delta_{jn} \delta_{km}
    </me>.
  </p>
  <p>
    You may plug this form into the expression on the left-hand side.
    You then obtain 2 terms, which you can evaluate separately.
    Summing over a delta eliminates one of its two indices:
    for example:
    <me>
      \sum_{j,k,m,n} \delta_{jm} \delta_{kn}  y_j y_m z_k z_n  = \sum_{j,k} y_j y_j z_k z_k
    </me>,
    since the only <m>m</m> term that contributes is <m>m=j</m>,
    and the only <m>n</m> term that contributes is <m>n=k</m>.
    From there, it's a short hop to the expression with inner products.
  </p>
  <p>
    In order to get the expression with <m>\sin \theta</m>,
    you will need the cosine formula for inner products
    (see <xref ref="sec_SigmaApp_RotationMatrix3D">Section</xref>).
  </p>
  <p>
    <xref ref="exercise_SigmaApp_sigmaAssoc">Exercise</xref>: Write matrices <m>G</m> and <m>H</m> from parts (b) and (c) in terms of <m>A,B</m>,
    and <m>C</m>.
  </p>
  <p>
    <xref ref="exercise_SigmaApp_trace3">Exercise</xref>: Notice that the product <m>{AB}</m> is in both terms.
    So for simplicity you can define <m>M := AB</m>,
    and use a previous result.
  </p>
  <p>
    <xref ref="exercise_SigmaApp_linalg">Exercise</xref>(a) You don't need summation notation here,
    just use basic properties of inverses. (b): Use one of the previous exercises.
  </p>
  <p>
    <xref ref="exercise_SigmaApp_KLC">Exercise</xref>: There are two possibilities to consider,
    <m>i=j</m> and <m>i \neq j</m>.
  </p>
  <p>
    <xref ref="exercise_SigmaApp_split">Exercise</xref>(a): Hint: Make a table for all possible values of <m>i,j,k</m>.
  </p>
  <p>
    <xref ref="exercise_SigmaApp_split">Exercise</xref>(b): Multiply the equation you found in (a) by <m>a_{ijk}</m> and sum over all <m>i,j,k</m>.
  </p>
  <p>
    <xref ref="exercise_SigmaApp_detTrans">Exercise</xref>: Notice that
    <m>a_{1, \phi(1)} a_{2, \phi(2)} a_{3, \phi(3)}</m> is equal to <m>a_{\phi^{-1}(1), 1} a_{\phi^{-1}(2), 2} a_{\phi^{-1}(3), 3}</m>,
    and that sign(<m>\phi</m>) is equal to sign(<m>\phi^{-1}</m>).
  </p>
  <p>
    <xref ref="exercise_SigmaApp_EqualZero">Exercise</xref>: Replace
    <m>\epsilon_{xy}</m> with <m>-\epsilon_{yx}</m>,
    and show that the expression is equal to the negative of itself.
    (Alternatively, you can just verify the two cases:
    <m>i=j=1</m> and <m>i=j=2</m>.)
  </p>
</section>