<section xml:id="sec_SigmaNotation_Properties">
  <title>Algebraic rules for Sigmas</title>
  <introduction>
    <p>
      As with any algebraic notation,
      there are rules that allow us to do algebraic manipulations with expressions that involve sigmas.
      In this section, we explore some of these rules.
    </p>
  </introduction>
  <subsection>
    <title>Constant multiples, sums, and products of sums</title>
    <p>
      Many of the rules for manipulating sigmas follow from the commutative law of addition and the associative and distributive laws for addition and multiplication.
      To motivate these rules,
      we will look at simple examples and then generalize.
    </p>
    <p>
      Let's first consider the example:
      <me>
        \sum_{i=0}^{5}2i
      </me>
    </p>
    <p>
      We know this is the sigma notation for <m>2\cdot1+2\cdot2+2\cdot3+2\cdot4+2\cdot5</m>.
      Using the distributive property of addition and multiplication of integers,
      we know this sum is the same as <m>2\cdot(1+2+3+4+5)</m>.
      Now we convert the sum in the parenthesis to sigma notation to yield
      <me>
        2\cdot\sum_{i=0}^{5}i
      </me>.
    </p>
    <p>
      The same argument could be used for any sum multiplied by any constant.
      We can write this rule as:
      <men>
        \sum_{i=a}^{b} c \cdot d_i = c \cdot \sum_{i=a}^{b}  d_i
      </men>,
      where <m>c</m> denotes an arbitrary constant and <m>d_i</m> represents the term of the sum corresponding to index <m>i</m>.
      Suppose next we take the sum of two sums and combine them into a single sum using the commutative law:
      <md>
        <mrow>\sum_{i=0}^4 i + \sum_{j=0}^4 2^j \amp =  (0+1+2+3+4) + (2^0 + 2^1 + 2^2 + 2^3 + 2^4)</mrow>
        <mrow>\amp = (0+2^0) + (1+2^1) + (2+2^2) + (3+2^3) + (4+2^4)</mrow>
        <mrow>\amp = \sum_{i=0}^4 (i + 2^i)</mrow>
      </md>.
    </p>
    <p>
      Applying the same process to an arbitrary sum of two sums gives:
      <men xml:id="eq_combineSums">
        \sum_{i=0}^n x_i + \sum_{j=0}^n y_j =\sum_{i=0}^n (x_i + y_i)
      </men>
    </p>
    <p>
      Now let's look at an example of a product of two sums.
      Using the commutative law of addition and the distributive law repeatedly, we have:
      <md>
        <mrow>\amp  \left(\sum_{i=1}^4 i\right)\left(\sum_{j=1}^3 \frac{1}{j}\right)  = (1+2+3+4)(1 + 1/2 + 1/3)</mrow>
        <mrow>\amp  = 1(1 + 1/2 + 1/3) + 2(1 + 1/2 + 1/3) + 3(1 + 1/2 + 1/3) + 4(1 + 1/2 + 1/3)</mrow>
        <mrow>\amp  = 1\cdot 1 + 1\cdot (1/2) + 1 \cdot (1/3) + 2 \cdot 1 + 2 \cdot (1/2) + 2 \cdot (1/3) + 3 \cdot 1 + 3 \cdot (1/2) + 3 \cdot (1/3)</mrow>
        <mrow>\amp  \qquad + 4 \cdot 1 + 4 \cdot (1/2) + 4 \cdot (1/3)</mrow>
      </md>.
    </p>
    <p>
      We see that the product of a sum of 4 terms with a sum of 3 terms gives a sum of <m>4\cdot 3 = 12</m> terms.
      Furthermore,
      the 12 terms consist of all possible products of (a term from the first sum) times (a term from the second sum).
      We introduce the following notation to describe this:
      <me>
        \left(\sum_{i=1}^4 i\right)\left(\sum_{j=1}^3 \frac{1}{j}\right) = \sum_{i=1}^4\sum_{j=1}^3 \frac{i}{j}
      </me>.
    </p>
    <p>
      We may generalize the above example to the product of two arbitrary sums as follows:
      <men xml:id="eq_prodSums">
        \begin{aligned}\left(\sum_{i=1}^n x_i\right)\left(\sum_{j=1}^m y_j\right)  \amp = \sum_{i=1}^n \left( x_i\left(\sum_{j=1}^m y_j\right)\right) \\ \amp =  \sum_{i=1}^n \sum_{j=1}^m x_i y_j \end{aligned}
      </men>
    </p>
    <exercise>
      <statement>
        <p>
          In view of Equation<nbsp/><xref ref="eq_combineSums"/>, one might suppose that the following is true:
          <me>
            \left(\sum_{i=0}^n x_i \right) \cdot  \left(  \sum_{i=0}^n y_i \right) \stackrel{?}{=} \sum_{i=0}^n x_i y_i
          </me>
          <ol type="a">
            <li>
              <p>
                Is this statement always true?
                If not, give an example of sequences <m>\{x_i\}</m> and <m>\{y_i\}</m> such that the equality does not hold.
              </p>
            </li>
            <li>
              <p>
                Is this statement <em>ever</em> true?
                If possible,
                give an example of sequences <m>\{x_i\}</m> and <m>\{y_i\}</m> such that the equality <em>does</em> hold.
              </p>
            </li>
          </ol>
        </p>
      </statement>
    </exercise>
    <p>
      We may now use Equations <xref ref="eq_combineSums"/> and <xref ref="eq_prodSums"/> to break down complicated multiple sums into simpler parts which may be evaluated more easily:
    </p>
    <exercise>
      <statement>
        <p>
          Given that <m>\sum_{i=1}^{20} i = 210</m> and
          <m>\sum_{i=1}^{20} i^2 = 2870</m>, Evaluate the following double sums:
          <ol type="a">
            <li>
              <p>
                <me>
                  \sum_{i=1}^{20} \sum_{j=1}^{20} (i+j)^2
                </me>
              </p>
            </li>
            <li>
              <p>
                <me>
                  \sum_{i=1}^{20} \sum_{j=1}^{20} (i-j)^2
                </me>
              </p>
            </li>
            <li>
              <p>
                <me>
                  \sum_{i=1}^{20} \sum_{j=1}^{20} (3i-4j)^2
                </me>
              </p>
            </li>
          </ol>
        </p>
      </statement>
    </exercise>
  </subsection>
</section>