<section xml:id="sec_Functions_Inverse">
  <title>Inverse functions<nbsp/><nbsp/></title>
  <figure>
    <video youtubeplaylist="PL2uooHqQ6T7PW5na4EX8rQX2WvBBdM8Qo"/>
  </figure>
  <subsection xml:id="subsec_Functions_Inverse_ConceptAndDefinition">
    <title>Concept and definition</title>
    <p>
      The word "inverse" commonly means something that is
      <q>backwards</q>
      or
      <q>opposite</q>
      to something else.
      So an inverse of a function should be a function that is somehow backwards or opposite to the original function.
      You have actually seen inverse functions many times before,
      perhaps without realizing it.
    </p>
    <example>
      <statement>
        <p>
          In <xref ref="example_Functions_5x-7BijectionEg">Example</xref>,
          we showed that <m>f(x) = 5x - 7</m> is a bijection.
          A quick look at the proof reveals that the formula
          <me>
            x =  \frac{y+7}{5}
          </me>
          plays a key role.
          This formula is obtained by replacing <m>f(x)</m> in
          <m>f(x) = 5x - 7</m> with <m>y</m>, and solving for <m>x</m>.
        </p>
        <p>
          In order to see <m>x = \frac{y+7}{5}</m> as an
          <q>inverse function,</q>
          we translate into the language of functions,
          by defining <m>g \colon \mathbb{R} \to \mathbb{R}</m> by <m>g(y) = (y+7)/5</m>.
          Then the above assertion can be restated as:
          <md>
            <mrow>y = f(x) \eiff x = g(y) </mrow>
          </md>.
        </p>
        <p>
          This tells us that <m>g</m> does exactly the opposite of what<nbsp/><m>f</m> does:
          if <m>f</m> takes <m>x</m> to<nbsp/><m>y</m>,
          then <m>g</m> takes <m>y</m> to<nbsp/><m>x</m>.
          We will say that <m>g</m> is an
          <q>inverse</q>
          of<nbsp/><m>f</m>.
        </p>
      </statement>
    </example>
    <example>
      <statement>
        <p>
          Let <m>f \colon \mathbb{R}^+ \rightarrow \mathbb{R}^+</m> be defined by:
          <m>f(x) = x^2</m>.
          We may define <m>g \colon \mathbb{R}^+ \to \mathbb{R}^+</m> by:
          <m>g(y) = \sqrt{y}</m>.
          Note that in this case the domains and ranges are restricted to
          <em>positive</em> real numbers.
          Given this restriction, by the definition of square root we have
          <me>
            y = x^2 \eiff  x = \sqrt{y}
          </me>.
        </p>
        <p>
          In view of the definitions of <m>f</m> and <m>g</m>,
          we may see that this is the same formula as in the previous example:
          <m>y = f(x) \eiff x = g(y)</m>.
        </p>
      </statement>
    </example>
    <example>
      <statement>
        <p>
          In the previous examples,
          the domain and codomain were the same<ndash/>but this doesn't always have to be the case.
          Let <m>f \colon \mathbb{R} \rightarrow \mathbb{R}^+</m> be defined by <m>f(x) = e^x</m>.
          We may define <m>g \colon \mathbb{R}^+ \to \mathbb{R}</m> by <m>g(y) = \ln (y)</m>,
          where 'ln' denotes the natural logarithm function.
          Here we also obtain <m>y = f(x) \eiff x = g(y)</m> as before,
          as long as <m>x</m> is in the domain of <m>f</m> and <m>y</m> is in the domain of <m>y</m>.
        </p>
      </statement>
    </example>
    <p>
      The <m>\eiff</m> statement which has popped up in the last three examples can be re-expressed as a pair of equations involving <m>f</m> and <m>g</m>,
      as the following proposition shows:
    </p>
    <proposition xml:id="proposition_Functions_xgyInverseExer">
      <statement>
        <p>
          Suppose that <m>f \colon X \to Y</m> and
          <m>g \colon Y \to X</m> are functions such that
          <me>
            \forall x \in X, \forall y \in Y, \bigl(y = f(x) \eiff x = g(y) \bigr)
          </me>.
        </p>
        <p>
          Then the following statements are also true:
          <ol type="a">
            <li xml:id="x_g_y___InverseExer-g_f_x__">
              <p>
                <m>g \bigl( f(x) \bigr) = x</m> for all <m>x \in X</m>. and
              </p>
            </li>
            <li xml:id="x_g_y___InverseExer-f_g_y__">
              <p>
                <m>f \bigl( g(y) \bigr) = y</m> for all <m>y \in Y</m>,
              </p>
            </li>
          </ol>
        </p>
      </statement>
    </proposition>
    <p>
      We will furnish the proof of (a),
      while the proof of (b) is left as an exercise.
    </p>
    <proof>
      <p>
        The proof of (a) runs as follows.
        Suppose that <m>y = f(x) \eiff x = g(y)</m> for all <m>x,y</m> in the respective domains of <m>f</m> and <m>g</m>.
        Then for any <m>x \in X</m>, we may define <m>z</m> as <m>z = f(x)</m>.
        By the <m>\eiff</m> statement it follows that <m>x = g(z)</m>.
        But then we may substitute the first equation into the second and obtain <m>g(f(x)) = x</m>.
        Since <m>x</m> was an arbitrary element of <m>X</m>,
        it follows that <m>g(f(x)) = x</m> for all <m>x \in X</m>.
      </p>
    </proof>
    <exercise xml:id="exercise_Functions_88">
      <statement>
        <p>
          Prove part (b) of <xref ref="proposition_Functions_xgyInverseExer">Proposition</xref>.
        </p>
      </statement>
    </exercise>
    <exercise xml:id="exercise_Functions_conv88">
      <statement>
        <p>
          Prove the converse of <xref ref="proposition_Functions_xgyInverseExer">Proposition</xref>.
          That is, given that
          <me>
            g \bigl( f(x) \bigr) = x \text{ for all }  x \in X  \text{ and }   f \bigl( g(y) \bigr) = y \text{ for all } y \in Y
          </me>,
          it follows that
          <me>
            \forall x \in X, \forall y \in Y, \bigl(y = f(x) \eiff x = g(y) \bigr)
          </me>.
        </p>
      </statement>
    </exercise>
    <p>
      Finally, we can give the definition of an inverse function:
    </p>
    <definition>
      <statement>
        <p>
          {invfna} Suppose <m>f \colon X \to Y</m> and <m>g \colon Y \to X</m> are functions.
          We say that <m>g</m> is an <term>inverse function </term>
              <idx><h>Inverse</h><h>function</h></idx>
              <idx><h>Function</h><h>inverse of</h></idx>
          for the function<nbsp/><m>f</m> if and only if:
          <ol type="a">
            <li>
              <p>
                <m>f \bigl( g(y) \bigr) = y</m> (in other words,
                <m>f \compose g(y) = y</m>) for all <m>y \in Y</m>, and
              </p>
            </li>
            <li>
              <p>
                <m>g \bigl( f(x) \bigr) = x</m> (in other words,
                <m>g \compose f(x) = x</m>) for all <m>x \in X</m>.
              </p>
            </li>
          </ol>
        </p>
      </statement>
    </definition>
    <example>
      <statement>
        <p>
          The husband of the wife of any married man is the man himself <mdash/> in other words,
          <me>
            \var{husband}\bigl( \var{wife} (y) \bigr) = y
          </me>.
        </p>
        <p>
          Also, the wife of the husband of any married woman is the woman herself, so that
          <me>
            \var{wife}\bigl( \var{husband} (x) \bigr) = x
          </me>.
        </p>
        <p>
          It follows that the <m>\var{wife}</m> function is an inverse of the<nbsp/><m>\var{husband}</m> function.
          In fact, it's pretty clear that <m>\var{husband}</m> is the <em>only</em>
          inverse of <m>\var{wife}</m>.
        </p>
      </statement>
    </example>
    <exercise xml:id="exercise_Functions_VerifyInverseExers">
      <statement>
        <p>
          In each case,
          use <xref ref="definition_Functions_invfna">Definition</xref>
          to determine whether <m>g</m> is an inverse of<nbsp/><m>f</m>.
          <ol type="a">
            <li xml:id="VerifyInverseExers-_9x-6_">
              <p>
                <m>f \colon \real \to \real</m> is defined by <m>f(x) = 9x - 6</m> and
                <m>g \colon \real \to \real</m> is defined by <m>g(y) = (y + 6)/9</m>.
              </p>
            </li>
            <li xml:id="VerifyInverseExers-_x_2_">
              <p>
                <m>f \colon \real^+ \to \real^+</m> is defined by <m>f(x) =2x^2</m> and
                <m>g \colon \real^+ \to \real^+</m> is defined by <m>g(y) = \sqrt{y}/2</m>.
              </p>
            </li>
            <li xml:id="VerifyInverseExers-_1_x_">
              <p>
                <m>f \colon \real^+ \to \real^+</m> is defined by <m>f(x) = 2/x</m> and
                <m>g \colon \real^+ \to \real^+</m> is defined by <m>g(y) = 2/y</m>.
              </p>
            </li>
            <li xml:id="VerifyInverseExers-_sqrt_x_1_-1_">
              <p>
                <m>f \colon \real^+ \to \real^+</m> is defined by <m>f(x) = \sqrt{x+1} - 1</m> and
                <m>g \colon \real^+ \to \real^+</m> is defined by <m>g(y) = y^2 + 2y</m>.
              </p>
            </li>
          </ol>
        </p>
      </statement>
    </exercise>
  </subsection>
  <subsection xml:id="subsec_Function_Inverse_DoFuncHaveInverses">
    <title>Which functions have inverses?</title>
    <p>
      It turns out that most functions do
      <em>not</em> have inverses.
    </p>
    <exercise xml:id="exercise_Functions_92">
      <statement>
        <p>
          Which of the functions depicted in <xref ref="arrowontofig">Figure</xref> have inverses?
        </p>
      </statement>
    </exercise>
    <p>
      From the previous exercise, you may have guessed the following rule:
    </p>
    <proposition xml:id="proposition_Functions_InverseBijection">
      <statement>
        <p>
          Suppose <m>f\colon X \to Y</m>.
          Then <m>f</m> has an inverse
          <m>g \colon Y \to X</m> if and only if <m>f</m> is a bijection.
              <idx><h>Function</h><h>as a bijection</h></idx>
              <idx><h>Bijection</h><h>relation to inverse functions</h></idx>
              <idx><h>Inverse function</h><h>relation to bijection</h></idx>
        </p>
      </statement>
    </proposition>
    <p>
      This is another
      <q>if and only if</q>
      proof, so it must be proved in both directions.
      We will prove the forward direction of this proposition.
      You will prove the reverse direction.
      The forward direction says that if
      <m>f \colon X \to Y</m> has an inverse <m>g \colon Y \to X</m>,
      then <m>f</m> is a bijection.
      In other words we must assume the first statement,
      and from that prove that <m>f</m> is one-to-one and onto.
    </p>
    <proof>
      <p>
        <em>(forward direction)</em> Assume there is a function
        <m>g \colon Y \to X</m> that is an inverse of<nbsp/><m>f</m>.
        Then by the definition of an inverse function,
        <ol type="a">
          <li>
            <p>
              <m>f \bigl( g(y) \bigr) = y</m> for all <m>y \in Y</m>, and
            </p>
          </li>
          <li>
            <p>
              <m>g \bigl( f(x) \bigr) = x</m> for all <m>x \in X</m>.
            </p>
          </li>
        </ol>
      </p>
      <p>
        Suppose then that <m>f(x_1) = f(x_2)</m> for some <m>x_1, x_2 \in X</m>.
        Then since <m>g</m> is a function we have
        <me>
          g \bigl( f(x_1) \bigr) = g \bigl( f(x_2) \bigr)
        </me>
      </p>
      <p>
        Therefore by (b), <m>x_1 = x_2</m>.
        Hence <m>f</m> is one-to-one.
      </p>
      <p>
        Now suppose <m>y \in Y</m>.
        Then since <m>g</m> is a function,
        there exists a unique <m>x \in X</m> such that <m>g(y) = x</m>.
        Substituting into (a) we get
        <me>
          f (x) = y
        </me>.
      </p>
      <p>
        Therefore <m>\forall y \in Y, \exists x \in X \mbox{ s.t. } f(x) = y</m>.
        Hence <m>f</m> is onto.
        So <m>f</m> is both one-to-one and onto:
        thus <m>f</m> is a bijection.
      </p>
    </proof>
    <exercise xml:id="exercise_Functions_InverseBijection2">
      <statement>
        <p>
          Prove the reverse direction of <xref ref="proposition_Functions_InverseBijection">Proposition</xref>. (*Hint*)
        </p>
      </statement>
    </exercise>
    <p>
      A function that has an inverse is said to be <em>invertible</em>.
          <idx><h>Function</h><h>invertible</h></idx>
          <idx><h>Invertible function</h></idx>
      The following exercise deals with a very important class of invertible functions/bijections.
    </p>
    <exercise xml:id="exercise_Functions_inverMod">
      <statement>
        <p>
          Given a number <m>a \in \mathbb{Z}_n</m>,
          consider the function <m>f_a: \mathbb{Z}_n \rightarrow \mathbb{Z}_n</m> given by <m>f_a(m) = a \odot m</m>.
          <ol type="a">
            <li>
              <p>
                Show that the function <m>f_6</m> defined on
                <m>\mathbb{Z}_7</m> is a bijection by finding an inverse of <m>f_6</m>.
              </p>
            </li>
            <li>
              <p>
                For the six numbers <m>a=0,1,2,3,4,5</m> in <m>\mathbb{Z}_6</m>,
                which of these give bijections for <m>f_a</m>?
                <em>Explain</em> your answer.
                Suppose that <m>a \in \mathbb{Z}_n</m> is relatively prime to <m>n</m>.
                Show that in this case,
                <m>f_a:\mathbb{Z}_n \rightarrow \mathbb{Z}_n</m> is a bijection
                (you may want to refer to <xref ref="subsec_ModularArithmetic_diophantine">Section</xref>). (*Hint*)
              </p>
            </li>
            <li>
              <p>
                Suppose that <m>a \in \mathbb{Z}_n</m> such that <m>ax \equiv 1 \pmod{n}</m> does <em>not</em>
                have an integer solution <m>x</m>.
                Show that in this case,
                <m>f_a:\mathbb{Z}_n \rightarrow \mathbb{Z}_n</m> is
                <em>not</em> a bijection. (*Hint*)
              </p>
            </li>
          </ol>
        </p>
      </statement>
    </exercise>
    <p>
      We close out this section with several exercises that prove various properties of inverses.
    </p>
    <exercise xml:id="exercise_Functions_InverseUniqueExers">
      <statement>
        <ol type="a">
          <li xml:id="InverseUniqueExers-bij">
            <p>
              Prove that any inverse of a bijection is a bijection.
            </p>
          </li>
          <li xml:id="InverseUniqueExers-unique">
            <p>
              Show that the inverse of a function is <em>unique</em>:
              if <m>g_1</m> and<nbsp/><m>g_2</m> are inverses of<nbsp/><m>f</m>,
              then <m>g_1 = g_2</m>. (*Hint*)
            </p>
          </li>
        </ol>
      </statement>
    </exercise>
    <remark>
      <ol type="a">
        <li>
          <p>
            <xref ref="exercise_Functions_InverseUniqueExers">Exercise</xref>
            is key because it enables us to talk about
            <em>the</em> inverse of a function,
            since there is never more than one inverse.
            We will use the special notation <m>f^{-1}</m><idx><h>Inverse function</h><h>notation</h></idx> to denote the inverse of the function <m>f</m>.
          </p>
        </li>
        <li>
          <p>
            According to <xref ref="definition_Functions_functionDef">Definition</xref>,
            any function can be specified by a set of ordered pairs.
            That is, if <m>f:X \rightarrow Y</m>,
            we can also write <m>f \subset X \times Y</m>,
            where for all <m>x \in X</m> there is a unique <m>y \in Y</m> such that <m>(x,y) \in f</m>.
            If <m>f</m> is a function that has an inverse,
            <m>f^{-1}</m> can also be expressed as a subset of <m>Y \times X</m>:
            <me>
              f^{-1} = \{\, (y,x) \mid (x,y) \in f \,\}
            </me>.
            This is simply a restatement of the fact that
            <me>
              y = f(x) \text{ iff }  x = f^{-1}(y)
            </me>.
          </p>
        </li>
      </ol>
    </remark>
    <definition>
      <statement>
        <p>
          {identityMap} For any set<nbsp/><m>A</m>,
          define the <term>identity map</term>
          <m>\Id_A \colon A \to A</m> by
          <m>\Id_A(a) = a</m> for every <m>a \in A</m>.
        </p>
      </statement>
    </definition>
    <p>
          <idx><h>Identity map</h></idx>
    </p>
    <exercise xml:id="exercise_Functions_IdAInverse">
      <statement>
        <ol type="a">
          <li>
            <p>
              Show that <m>\Id_A</m> is invertible.(*Hint*)
            </p>
          </li>
          <li>
            <p>
              Find the inverse of <m>\Id_A</m>.(*Hint*)
            </p>
          </li>
        </ol>
      </statement>
    </exercise>
    <exercise xml:id="exercise_Functions_InverseIdentityExers">
      <statement>
        <ol type="a">
          <li xml:id="InverseIdentityExers-InvOfComp">
            <p>
              Suppose <m>f \colon A \to B</m> and <m>g \colon B \to C</m> are bijections.
              Show that <m>(g \compose f)^{-1} = f^{-1} \compose g^{-1}</m>. (*Hint*)
            </p>
          </li>
          <li xml:id="InverseIdentityExers-Comp_Id">
            <p>
              Suppose <m>f \colon X \to Y</m> and <m>g \colon Y \to X</m>.
              Show that <m>g</m> is the inverse of<nbsp/><m>f</m> if and only if
              <me>
                f \compose g = \Id_Y \text{  and  } g \compose f = \Id_X
              </me>.
              (*Hint*)
            </p>
          </li>
          <li xml:id="InverseIdentityExers-InvOfInv">
            <p>
              Suppose <m>f \colon X \to Y</m> is a bijection.
              Show that the inverse of<nbsp/><m>f^{-1}</m> is<nbsp/><m>f</m>.
              That is, <m>(f^{-1})^{-1} = f</m>.
            </p>
          </li>
        </ol>
      </statement>
    </exercise>
  </subsection>
</section>