<section xml:id="sec_ModularArithmetic_Hints">
  <title>Hints for
  <q>Modular Arithmetic</q>
  exercises</title>
  <p>
    <xref ref="exercise_ModularArithmetic_eqproof">Exercise</xref>: Use the alternative definition of modular equivalence in <xref ref="proposition_ModularArithmetic_equivalence_alt">Proposition</xref>.
  </p>
  <p>
    <xref ref="exercise_ModularArithmetic_UPCSymbols">Exercise</xref>(f): Prove by contradiction:
    suppose the codes <m>d_1, d_2, \ldots d_{10}</m> and <m>e_1, e_2, \ldots e_{10}</m> are both valid,
    and suppose that all digits are equal except for the <m>n</m>'th digit
    (so <m>d_n \neq e_n</m>).
    There are two cases: (a) <m>n</m> is even; (b) <m>n</m> is odd.
    In case (a),
    show that this implies <m>e_n - d_n \equiv 0 \pmod{10}</m>,
    and derive a contradiction.
    Prove case (b) similarly.
  </p>
  <p>
    <xref ref="exercise_ModularArithmetic_ISBNCodes">Exercise</xref>(d): Use the fact that <m>10 \equiv -1 \pmod{11}</m>.
  </p>
  <p>
    <xref ref="exercise_ModularArithmetic_ISBNCodes">Exercise</xref>(i): Prove by contradiction: Suppose the codes
    <m>d_1, d_2, \ldots d_{10}</m> and <m>e_1, e_2, \ldots e_{10}</m> are both valid,
    and suppose that all digits are equal except for the <m>n</m>'th digit
    (so <m>d_n \neq e_n</m>).
    Show that <m>d_n - e_n</m> satisfies <m>(d_n - e_n)n \equiv 0 \pmod{11}</m>,
    and show that the only solution is <m>d_n - e_n = 0</m>.
  </p>
  <p>
    <xref ref="exercise_ModularArithmetic_ISBNCodes">Exercise</xref>(j): Suppose the code <m>d_1, d_2, \ldots d_{10}</m> is valid,
    and suppose the code is still valid when the digits <m>d_n</m> and <m>d_{n+1}</m> are exchanged.
    Write down two modular equations,
    and take the difference between the two modular equations.
    Use this to find an equation involving <m>d_n</m> and <m>d_{n+1}</m>.
  </p>
  <p>
    <xref ref="exercise_ModularArithmetic_modeq3">Exercise</xref>(c): Find a <em>negative</em>
    number that is equivalent to <m>856 \pmod{123}</m>.
  </p>
  <p>
    <xref ref="exercise_ModularArithmetic_ModPower">Exercise</xref>(a): Let <m>m=\ell</m> and <m>b=a</m>.
    Check the conditions of the proposition still hold,
    and apply the proposition.
  </p>
  <p>
    <xref ref="exercise_ModularArithmetic_ops">Exercise</xref>(a): You will need to use <xref ref="proposition_ModularArithmetic_number_remainder">Proposition</xref> twice.
  </p>
  <p>
    <xref ref="exercise_ModularArithmetic_52">Exercise</xref>: Use the definitions of <m>\oplus</m> and <m>\odot</m>.
  </p>
  <p>
    <xref ref="exercise_ModularArithmetic_53">Exercise</xref>: Be careful about 0!
  </p>
  <p>
    <xref ref="exercise_ModularArithmetic_58">Exercise</xref>(b)(i): Use the fact that <m>0 \lt a \lt n</m>.
  </p>
  <p>
    <xref ref="exercise_ModularArithmetic_diophant">Exercise</xref>(a): The left-hand side is always even,
    no matter what <m>m</m> and <m>n</m> are.
  </p>
  <p>
    <xref ref="exercise_ModularArithmetic_prop74">Exercise</xref>: Use <xref ref="proposition_ModularArithmetic_Lin_comb">Proposition</xref>.
  </p>
  <p>
    <xref ref="exercise_ModularArithmetic_propiff">Exercise</xref>: Use <xref ref="proposition_ModularArithmetic_74">Proposition</xref>.
  </p>
  <p>
    <xref ref="exercise_ModularArithmetic_EuclidLemmaProof">Exercise</xref>(a): Use <xref ref="proposition_ModularArithmetic_74">Proposition</xref>.<nbsp/><nbsp/><nbsp/><nbsp/>(b):
    <m>p</m> must divide the left-hand side of the multiplied equation (explain why).<nbsp/><nbsp/><nbsp/><nbsp/>(c): Consider two cases (I) <m>a</m> is relatively prime to <m>p</m>; (II) <m>a</m> is not relatively prime to <m>p</m>.
  </p>
  <p>
    <xref ref="exercise_ModularArithmetic_93">Exercise</xref>: Use <xref ref="proposition_ModularArithmetic_mod_eq_solution">Proposition</xref>.
  </p>
  <p>
    <xref ref="exercise_ModularArithmetic_94">Exercise</xref>: Use the previous exercise.
  </p>
  <p>
    <xref ref="exercise_ModularArithmetic_congruence">Exercise</xref>(b): If <m>y</m> is a particular solution to <m>ax \equiv b \pmod 3</m>,
    then <m>x=y+3k</m> is also a solution.
    Similarly, if <m>z</m> is a particular solution to <m>cx \equiv d \pmod 7</m>,
    then <m>x=z+7\ell</m> is also a solution.
    Set the two expressions equal,
    and show there is always a solution for <m>k, \ell</m> regardless of the values of <m>y,z</m>.
  </p>
  <p>
    <xref ref="exercise_ModularArithmetic_congruence">Exercise</xref>
    (c): Follow the method used in the Chinese Remainder Theorem,
    and for each modular equivalence obtained show that a solution exists.
  </p>
  <p>
    <xref ref="exercise_ModularArithmetic_congruence">Exercise</xref>
    (d): Suppose that <m>x</m> and <m>y</m> are both solutions to the given pair of congruences.
    Show that <m>x-y \equiv 0 \pmod{m}</m> and <m>x-y \equiv 0 \pmod{n}</m>.
    This implies that both <m>m</m> and <m>n</m> divide <m>x-y</m>
    (explain why).
  </p>
</section>