<section xml:id="sec_Polynomials_ExoticPolynomials">
  <title>More exotic polynomials</title>
  <introduction>
    <p>
      So far we've performed algebraic operations on polynomials with integer,
      rational, real, or complex coefficients.
      We may identify different sets of polynomials according to the type of coefficient used.
      For instance we may define:
      <ul>
        <li>
          <p>
            <m>\mathbb{Z}[x]</m> is the set of polynomials in the variable <m>x</m> with integer coefficients;
          </p>
        </li>
        <li>
          <p>
            <m>\mathbb{Q}[x]</m> is the set of polynomials in the variable <m>x</m> with rational coefficients;
          </p>
        </li>
        <li>
          <p>
            <m>\mathbb{R}[x]</m> is the set of polynomials in the variable <m>x</m> with real coefficients;
          </p>
        </li>
        <li>
          <p>
            <m>\mathbb{C}[x]</m> is the set of polynomials in the variable <m>x</m> with complex coefficients.
          </p>
        </li>
      </ul>
    </p>
    <p>
      We refer to <m>\mathbb{Z}[x]</m> as
      <q>the set of polynomials over <m>\mathbb{Z}</m></q>, <m>\mathbb{Q}[x]</m> as
      <q>the set of polynomials over <m>\mathbb{Q}</m></q>, and so on.
    </p>
    <p>
      However, we can generalize polynomials far beyond these cases.
      In this section,
      we introduce several new types of polynomials and define arithmetic operations
      (addition and multiplication)
      on these new types.
      In order to do this,
      we'll make use of the summation notation formulas in the last section (reproduced here for convenience):
      <me>
        p(x)  = \sum^{M}_{m=0} a_m x^m ; \qquad q(x)  = \sum^{N}_{n=0} b_n x^n
      </me>,
      <md>
        <mrow>p(x) + q(x) \amp =  \sum_{k=0}^{\max(M,N)} (a_k + b_k) x^k,</mrow>
        <mrow>p(x) q(x) \amp = \sum_{k=0}^{M+N} c_k x^k, \text{ where } c_k=  \sum_{j = 0}^k a_j b_{k - j}</mrow>
      </md>.
    </p>
    <p>
      We'll just need to replace conventional addition and multiplication
      (using real or complex numbers)
      with other addition and multiplication operations that are appropriate to the coefficients that we are working with.
    </p>
  </introduction>
  <subsection xml:id="subsec_Polynomials_ExoticPolynomials_PolynomialsZn">
    <title>Polynomials over <m>\mathbb{Z}_n</m></title>
    <p>
          <idx><h>Polynomials</h><h>over <m>\mathbb{Z}_n</m></h></idx>
      Consider first <m>\mathbb{Z}_n[x]</m>, where <m>\mathbb{Z}_n</m> denotes the integers mod <m>n</m>.
      For example,
      two polynomials <m>p(x)</m> and <m>q(x)</m> in <m>\mathbb{Z}_4[x]</m> are
      <md>
        <mrow>p(x) \amp  = 1+3x+x^3</mrow>
        <mrow>q(x) \amp  = 2+2x+3x^2+3x^3</mrow>
      </md>.
    </p>
    <p>
      In this case,
      we should consider the variable <m>x</m> as representing an unknown element in <m>\mathbb{Z}_4</m>,
      so the '+' operation in these expressions should be interpreted as addition in <m>\mathbb{Z}_4</m>.
      All operations on coefficients will also make use of addition mod <m>\mathbb{Z}_4</m>.
      So for polynomial addition we may use the above formulas for polynomial addition only use <m>+</m> in <m>Z_4</m> instead of ordinary <m>+</m>.
      For example,
      using <m>p(x)</m> and <m>q(x)</m> defined above we have:
      <md>
        <mrow>p(x) + q(x) \amp =(1+ 2)+(3+ 2)x+(0+ 3)x^2+ (1+ 3)x^3</mrow>
        <mrow>\amp = 3+x+3x^2</mrow>
      </md>.
    </p>
    <p>
      To multiply, we can use the same strategy,
      namely, use the previous formula for polynomial multiplication,
      but replace both <m>+</m> and <m>\cdot</m> with their counterparts in <m>Z_4</m>.
      Alternatively,
      we may use the distributive law as in <xref ref="sec_Polynomials_PolynomialArithmetic">Section</xref>,
      with the understanding that we are distributing modular multiplication over modular addition.
      As before, we group together all terms with like powers of <m>x</m> and use modular arithmetic to combine these terms into a single term.
      The result is:
      <md>
        <mrow>p(x)  q(x)  =  \amp 1\cdot 2+(3 \cdot 2 + 1 \cdot 2)x+(3 \cdot 2 +  1 \cdot 3)x^2+</mrow>
        <mrow>\amp (1\cdot 2 + 3\cdot 3 +  1 \cdot 3)x^3+ (1\cdot 2 +  3\cdot 3)x^4 +</mrow>
        <mrow>\amp (1 \cdot 3)x^5+ (1 \cdot 3)x^6</mrow>
        <mrow>= \amp 2+1x^2 + 2x^3+ 3x^4+ 3x^5+3x^6</mrow>
      </md>.
    </p>
    <exercise xml:id="exercise_Polynomials_poly7">
      <statement>
        <p>
          Compute the sum and product of <m>p(x)</m> and <m>q(x)</m>.
          <ol type="a">
            <li>
              <p>
                <m>p(x)=1+x+2x^2</m>,
                <m>q(x)=3x^2+x^3</m>,where both polynomials are in <m>\mathbb{Z}_5[x]</m>.
              </p>
            </li>
            <li>
              <p>
                <m>p(x)= 1+4x^2+3x^3+2x^4</m>, <m>q(x)=5+2x^2+x^3</m>,
                where both polynomials are in <m>\mathbb{Z}_6[x]</m>.
              </p>
            </li>
          </ol>
        </p>
      </statement>
    </exercise>
    <p>
      It turns out that <m>\mathbb{Z}_2[x]</m> in particular is of great practical use
      (in polynomial codes),
      so we include some exercises to get you warmed up for what's coming.
    </p>
    <exercise xml:id="exercise_Polynomials_poly6">
      <statement>
        <p>
          Compute the sum and product of <m>p(x)</m> and <m>q(x)</m>,
          where both polynomials are in <m>\mathbb{Z}_2[x]</m>.
          <ol type="a">
            <li>
              <p>
                <m>p(x)= 1+ x +x^2</m>, <m>q(x)= 1+x+x^2+x^3</m>
              </p>
            </li>
            <li>
              <p>
                <m>p(x)= 1 + x^2+x^4</m>, <m>q(x)=x^2+x^3+x^4</m>.
              </p>
            </li>
            <li>
              <p>
                <m>p(x)= 1 +x+x^2+x^3+x^4</m>, <m>q(x)=p(x)</m>.
              </p>
            </li>
          </ol>
        </p>
      </statement>
    </exercise>
  </subsection>
  <subsection xml:id="subsec_Polynomials_ExoticPolynomials_nZ">
    <title>Polynomials over <m>n\mathbb{Z}</m></title>
    <p>
          <idx><h>Polynomials</h><h>over <m>n\mathbb{Z}</m></h></idx>
      Recall that <m>n\mathbb{Z}</m> consists of all integer multiples of <m>n</m>: for example, <m>5\mathbb{Z} = \{\ldots, -15,-10,-5,0,5,10,15,\ldots\}</m>.
      We may consider the set <m>n\mathbb{Z}[x]</m>,
      the set of all polynomials whose coefficents are all multiples of <m>n</m>.
      Certainly it is possible to add and multiply these polynomials,
      because any such polynomial is also in <m>\mathbb{Z}[x]</m>.
      But it is important to note that any sum or product of polynomials in
      <m>n\mathbb{Z}[x]</m> is also in <m>n\mathbb{Z}[x]</m>:
      in other words, <m>n\mathbb{Z}[x]</m> is <em>closed</em>
      under addition and multiplication.
    </p>
    <exercise xml:id="exercise_Polynomials_5Z">
      <statement>
        <ol type="a">
          <li>
            <p>
              Suppose that <m>p(x) = a_2 x^2 + a_1 x + a_0</m> and <m>q(x) = b_1 x + b_0</m>,
              and both <m>p(x)</m> and <m>q(x)</m> are elements of <m>5\mathbb{Z}[x]</m>.
              Prove that <m>p(x) + q(x)</m> and
              <m>p(x) q(x)</m> are also elements of <m>5\mathbb{Z}[x]</m>. (*Hint*)
            </p>
          </li>
          <li>
            <p>
              Repeat the proof of (a),
              except replace <m>5\mathbb{Z}[x]</m> with <m>n\mathbb{Z}[x]</m>,
              where <m>n</m> is an arbitrary positive integer.
            </p>
          </li>
          <li>
            <p>
              Repeat the proof of (b),
              except use general polynomials
              <m>p(x) = \sum_{j=1}^n a_jx^j</m> and <m>q(x) = \sum_{k=1}^m b_k x^k</m>.
            </p>
          </li>
        </ol>
      </statement>
    </exercise>
  </subsection>
  <subsection xml:id="subsec_Polynomials_ExoticPolynomials_PolynomialsR">
    <title>Polynomials over <m>\mathbb{R}[x]</m></title>
    <p>
          <idx><h>Polynomials</h><h>over <m>\mathbb{R}[x]</m></h></idx>
      Our next example is <m>\mathbb{R}[x][y]</m>, which represents polynomials in the variable <m>y</m> whose coefficients are polynomials in a different variable <m>x</m>.
      For example,
      the following two polynomials are elements of <m>\mathbb{R}[x][y]</m>:
      <md>
        <mrow>p(x,y) \amp  = (1+3x)+(1+x^2)y+(5x)y^2</mrow>
        <mrow>q(x,y) \amp  = (3x)+(2+2x)y+(4x^2)y^2</mrow>
      </md>.
    </p>
    <p>
      We may add them as follows:
      <md>
        <mrow>p(x,y) + q(x,y) \amp =((1+3x)+3x)+((1+x^2)+(2+2x))y+(5x+4x^2)y^2</mrow>
        <mrow>\amp = (1+6x)+(3+2x+x^2)y+(5x+4x^2 )y^2</mrow>
      </md>.
    </p>
    <p>
      We will multiply <m>p(x,y)</m> and <m>q(x,y)</m> using the summation formula for coefficients found in <xref ref="definition_Polynomials_defprodpoly">Definition</xref>.
      <md>
        <mrow>c_0 = \sum_{i = 0}^0 a_i b_{0 - i} = a_0b_0= (1+3x) \cdot (3x)= 3x+9x^2</mrow>
      </md>.
      <md>
        <mrow>c_1 = \sum_{i = 0}^1 a_i b_{0 - i} = a_0b_1+a_1b_0\amp = ((1+3x) \cdot (2+2x))+((1+x^2)\cdot (3x))</mrow>
        <mrow>\amp =(1+8x+6x^2)+(2+2x+2x^2+2x^3)</mrow>
        <mrow>\amp =3+10x+8x^2+2x^3</mrow>
      </md>.
      <md>
        <mrow>c_2 = \sum_{i = 0}^2 a_i b_{0 - i} = a_0b_2+a_1b_1+a_2b_0\amp =((1+3x) \cdot (4x^2))+(1+x^2)\cdot(2+2x)+((5x)\cdot(3x)</mrow>
        <mrow>\amp = (4x^2+12x^3)+(2+2x+2x^2+2x^3)+15x^2</mrow>
        <mrow>\amp =2+2x+21x^2+14x^3</mrow>
      </md>.
      <md>
        <mrow>c_3 = \sum_{i = 0}^3 a_i b_{0 - i} = a_1b_2+a_2b_1\amp = ((1+x^2) \cdot (4x^2))+((5x)\cdot(2+2x)</mrow>
        <mrow>\amp =  (4x^2+4x^4)+(10x+10x^2)</mrow>
        <mrow>\amp =10x+14x^2+4x^4</mrow>
      </md>.
    </p>
    <md>
      <mrow>c_4 = \sum_{i = 0}^4 a_i b_{0 - i} = a_2b_2= 5x \cdot 4x^2= 20x^3</mrow>
    </md>.
    <p>
      Therefore, we have the following:
      <md>
        <mrow>p(x,y)q(x,y)=\amp  c_0+c_1y+c_2y^2+c_3y^3+c_4y^4</mrow>
        <mrow>=\amp (3x+9x^2)+(3+10x+8x^2+2x^3)y+(2+2x+21x^2+14x^3)y^2</mrow>
        <mrow>\amp +(10x+14x^2+4x^4)y^3+(20x^3)y^4</mrow>
      </md>.
    </p>
    <exercise xml:id="exercise_Polynomials_poly8">
      <statement>
        <p>
          Compute the sum and product of <m>p(x,y)</m> and <m>q(x,y)</m> where:
        </p>
        <p>
          <m>p(x,y)= (1+8x)+(3-2x)y^2</m> and
        </p>
        <p>
          <m>q(x,y)= (5x+6x^2)y-(2+6x)y^2</m>
        </p>
      </statement>
    </exercise>
  </subsection>
  <subsection xml:id="subsec_Polynomials_ExoticPolynomials_Mn">
    <title>Polynomials over <m>\mathbb{M}_n</m></title>
    <p>
          <idx><h>Polynomials</h><h>over <m>\mathbb{M}_n</m></h></idx>
      Next we consider <m>\mathbb{M}_n[x]</m>, the set of polynomials in the variable <m>x</m> with coefficients that are <m>n{\times}n</m> matrices with real entries.
      Consider the two polynomials <m>p(x),
      q(x) \in \mathbb{M}_2[x]</m> given by:
      <me>
        p(x)=  \begin{bmatrix}-1 \amp  5  \\ -2 \amp  4 \end{bmatrix} +\begin{bmatrix}4 \amp  3 \\ 2 \amp  -4 \end{bmatrix} x+\begin{bmatrix}-1 \amp  0 \\ 2 \amp  1 \end{bmatrix} x^2
      </me>
      <me>
        q(x)=  \begin{bmatrix}4 \amp  2 \\ -3 \amp  6 \end{bmatrix} +\begin{bmatrix}2 \amp  -1 \\ 0 \amp  9 \end{bmatrix} x+\begin{bmatrix}9 \amp  -1 \\ 8 \amp  1 \end{bmatrix} x^2
      </me>
    </p>
    <p>
      We add <m>p(x)</m> and <m>q(x)</m> as follows:
      <md>
        <mrow>p(x) + q(x) =\amp \bigg( \begin{bmatrix} -1 \amp  5</mrow>
        <mrow>-2 \amp  4 \end{bmatrix} +\begin{bmatrix} 4 \amp  3</mrow>
        <mrow>2 \amp  -4 \end{bmatrix} x+\begin{bmatrix} -1 \amp  0</mrow>
        <mrow>2 \amp  1 \end{bmatrix} x^2\bigg)</mrow>
        <mrow>\amp +\bigg(\begin{bmatrix} 4 \amp  2</mrow>
        <mrow>-3 \amp  6 \end{bmatrix} +\begin{bmatrix} 2 \amp  -1</mrow>
        <mrow>0 \amp  9 \end{bmatrix} x+\begin{bmatrix} 9 \amp  -1</mrow>
        <mrow>8 \amp  1 \end{bmatrix} x^2\bigg)</mrow>
        <mrow>= \amp \bigg(\begin{bmatrix} -1 \amp  5</mrow>
        <mrow>-2 \amp  4 \end{bmatrix} +\begin{bmatrix} 4 \amp  2</mrow>
        <mrow>-3 \amp  6 \end{bmatrix}\bigg) +\bigg(\begin{bmatrix} 4 \amp  3</mrow>
        <mrow>2 \amp  -4 \end{bmatrix} +\begin{bmatrix} 2 \amp  -1</mrow>
        <mrow>0 \amp  9 \end{bmatrix}\bigg)x</mrow>
        <mrow>\amp +\bigg(\begin{bmatrix} -1 \amp  0</mrow>
        <mrow>2 \amp  1 \end{bmatrix} +\begin{bmatrix} 9 \amp  -1</mrow>
        <mrow>8 \amp  1 \end{bmatrix}\bigg) x^2</mrow>
        <mrow>=\amp \begin{bmatrix} 3 \amp  7</mrow>
        <mrow>-5 \amp  10 \end{bmatrix} +\begin{bmatrix} 6 \amp  2</mrow>
        <mrow>2 \amp  5 \end{bmatrix}x +\begin{bmatrix} 8 \amp  -1</mrow>
        <mrow>10 \amp  2\end{bmatrix}x^2</mrow>
      </md>.
    </p>
    <p>
      Again, we will use the summation formula for the coefficients to compute the product of <m>p(x)</m> and <m>q(x)</m>.
      <me>
        c_0 = \sum_{i = 0}^0 a_i b_{0 - i} = a_0b_0= \begin{bmatrix}-1 \amp  5 \\ -2 \amp  4 \end{bmatrix}  \cdot \begin{bmatrix}4 \amp  2 \\ -3 \amp  6 \end{bmatrix} = \begin{bmatrix}-19\amp  28\\ -20 \amp  20 \end{bmatrix}
      </me>.
      <md>
        <mrow>c_1 = \sum_{i = 0}^1 a_i b_{1 - i} = a_0b_1+a_1b_0\amp =\begin{bmatrix} -1 \amp  5</mrow>
        <mrow>-2 \amp  4 \end{bmatrix} \cdot \begin{bmatrix} 2 \amp  -1</mrow>
        <mrow>0 \amp  9 \end{bmatrix}+ \begin{bmatrix} 4 \amp  3</mrow>
        <mrow>2 \amp  -4 \end{bmatrix} \cdot\begin{bmatrix} 4 \amp  2</mrow>
        <mrow>-3 \amp  6 \end{bmatrix}</mrow>
        <mrow>\amp =\begin{bmatrix} -2 \amp  46</mrow>
        <mrow>-4 \amp  38 \end{bmatrix}+\begin{bmatrix} 7 \amp  26</mrow>
        <mrow>20 \amp  -20 \end{bmatrix}=\begin{bmatrix} 5 \amp  72</mrow>
        <mrow>16 \amp  18 \end{bmatrix}</mrow>
      </md>.
      <md>
        <mrow>c_2 = \sum_{i = 0}^2 a_i b_{2 - i} = a_0b_2+a_1b_1+a_2b_0\amp = \begin{bmatrix} -1 \amp  5</mrow>
        <mrow>-2 \amp  4 \end{bmatrix} \cdot \begin{bmatrix} 9 \amp  -1</mrow>
        <mrow>8 \amp  1 \end{bmatrix}+ \begin{bmatrix} 4 \amp  3</mrow>
        <mrow>2 \amp  -4 \end{bmatrix} \cdot\begin{bmatrix} 2 \amp  -1</mrow>
        <mrow>0 \amp  9 \end{bmatrix}</mrow>
        <mrow>\amp  +\begin{bmatrix} -1 \amp  0</mrow>
        <mrow>2 \amp  1 \end{bmatrix}\cdot \begin{bmatrix} 4 \amp  2</mrow>
        <mrow>-3 \amp  6 \end{bmatrix}</mrow>
        <mrow>\amp =\begin{bmatrix} 31 \amp  6</mrow>
        <mrow>14 \amp  6 \end{bmatrix}+\begin{bmatrix} 8 \amp  23</mrow>
        <mrow>4 \amp  -38 \end{bmatrix}+\begin{bmatrix} -4 \amp  -2</mrow>
        <mrow>5 \amp  10 \end{bmatrix}=\begin{bmatrix} 35 \amp  27</mrow>
        <mrow>23 \amp  -22 \end{bmatrix}</mrow>
      </md>.
      <md>
        <mrow>c_3 = \sum_{i = 0}^3 a_i b_{3 - i} = a_1b_2+a_2b_1\amp = \begin{bmatrix} 4 \amp  3</mrow>
        <mrow>2 \amp  -4 \end{bmatrix} \cdot \begin{bmatrix} 9 \amp  -1</mrow>
        <mrow>8 \amp  1 \end{bmatrix}+ \begin{bmatrix} -1 \amp  0</mrow>
        <mrow>2 \amp  1 \end{bmatrix} \cdot\begin{bmatrix} 2 \amp  -1</mrow>
        <mrow>0 \amp  9 \end{bmatrix}</mrow>
        <mrow>\amp =\begin{bmatrix} 60 \amp  -1</mrow>
        <mrow>-14 \amp  -6 \end{bmatrix}+\begin{bmatrix} -2 \amp  1</mrow>
        <mrow>4 \amp  7 \end{bmatrix}=\begin{bmatrix} 58 \amp  0</mrow>
        <mrow>-10 \amp  1 \end{bmatrix} </mrow>
      </md>.
    </p>
    <me>
      c_4 = \sum_{i = 0}^4 a_i b_{4 - i} = a_2b_2= \begin{bmatrix}-1 \amp  0 \\
      2 \amp  1
      \end{bmatrix}  \cdot \begin{bmatrix}9 \amp  -1\\
      8 \amp  1
      \end{bmatrix} =\begin{bmatrix}-9 \amp  1\\
      26 \amp  -1
      \end{bmatrix}
    </me>.
    <p>
      Therefore, we have the following:
      <md>
        <mrow>p(x)q(x) \amp =c_0+c_1x+c_2x^2+c_3x^3+c_4x^4</mrow>
        <mrow>\amp =\begin{bmatrix} -19 \amp  28</mrow>
        <mrow>-20 \amp  20 \end{bmatrix}+ \begin{bmatrix} 5 \amp  72</mrow>
        <mrow>16 \amp  18 \end{bmatrix}x+ \begin{bmatrix} 35 \amp 27</mrow>
        <mrow>23 \amp  -22 \end{bmatrix}x^2+ \begin{bmatrix} 58 \amp  0</mrow>
        <mrow>-10 \amp  1 \end{bmatrix}x^3+ \begin{bmatrix} -9 \amp  1</mrow>
        <mrow>26 \amp  -1 \end{bmatrix}x^4</mrow>
      </md>
    </p>
    <exercise xml:id="exercise_Polynomials_poly9">
      <statement>
        <p>
          Compute the sum and product of <m>p(x)</m> and <m>q(x)</m>, where:
          <me>
            p(x)=  \begin{bmatrix}1 \amp  2 \\ 3 \amp  4 \end{bmatrix} +\begin{bmatrix}1 \amp  0 \\ 2 \amp  4 \end{bmatrix} x+\begin{bmatrix}1 \amp  0 \\ 0 \amp  1 \end{bmatrix} x^2
          </me>
          <me>
            q(x)=  \begin{bmatrix}1 \amp  0 \\ 0 \amp  1 \end{bmatrix} +\begin{bmatrix}1 \amp  2 \\ 3 \amp  4 \end{bmatrix} x^2
          </me>
        </p>
      </statement>
    </exercise>
  </subsection>
</section>