<section xml:id="sec_Homomorphism_FirstIsomorphismTheorem">
  <title>The First Isomorphism Theorem</title>
  <p>
    There's one property that we observed in earlier sections of this chapter that we haven't proven so far, namely,
    the quotient group created by the kernel of a homomorphism is isomorphic to the image of the homomorphism.
    In order to do this,
    we'll need a clearer idea of how homomorphisms actually work.
    <xref ref="fig_homomorph3">Figure</xref>
    gives a schematic diagram of a general homomorphism <m>f</m> with kernel <m>K</m>.
  </p>
  <figure xml:id="fig_homomorph3">
    <caption>Homomorphism <m>f:G \rightarrow H</m> with kernel <m>K</m>.</caption>
    <image width="75%" source="images/homomorph3.png"/>
  </figure>
  <p>
    The figure shows the cosets of <m>K</m>,
    which form a partition of <m>G</m> as we showed in the Cosets chapter.
    These cosets can be thought of as elements of the quotient group <m>G/K</m>.
  </p>
  <p>
    The arrangement of arrows in the figure indicate that any two points in the same coset <m>gK</m> map to the same element of <m>H</m>.
    This is true because
    <me>
      f(gk) = f(g)f(k) = f(g)e' = f(g)\qquad (\text{ given that }  g \in G, k \in K)
    </me>.
  </p>
  <p>
    This implies that we can actually define a function <m>F</m> from <m>G/K</m> to <m>H</m> as follows:
    <me>
      F(gK) = f(g)
    </me>.
  </p>
  <p>
    The function is well-defined because if
    <m>g'K = gK</m> then <m>F(g'K) = f(g') = f(g) = F(gK)</m>.
  </p>
  <p>
    So what's the point?
    It turns out that this function <m>F</m> is exactly the isomorphism that we're looking for.
    We've already shown that it's well-defined:
    all that's left is to show that it's one-to-one and onto,
    and that it preserves the operation.
    We state these results as a proposition.
  </p>
  <proposition xml:id="proposition_Homomorphism_FirstIsoTheorem">
    <statement>
      <p>
        (<em>First Isomorphism Theorem</em>) <idx><h>First Isomorphism Theorem</h><h>for groups</h></idx>
      </p>
      <p>
        Suppose <m>f : G \rightarrow H</m> is a homomorphism with <m>K =\ker f</m>.
        Let the function <m>F: G/K \rightarrow f(G)</m> be defined according to <m>F(gK) = f(g)</m>.
        Then <m>F</m> is an isomorphism.
      </p>
    </statement>
  </proposition>
  <proof>
    <p>
      As mentioned above, we only need to show that <m>F</m> is 1-1, onto,
      and preserves the operation.
      <ul>
        <li>
          <p>
            1-1: Suppose that <m>F(g_1K) = F(g_2K)</m>.
            Then according to the definition of <m>F</m>,
            this means that <m>f(g_1) = f(g_2)</m>.
            From this we obtain (using the homomorphism property of <m>f</m>):
            <me>
              f(g_1^{-1}g_2)) = f(g_1^{-1})f(g_2) =  f(g_1)^{-1}f(g_2) = f(g_1)^{-1}f(g_1) = e'  \implies g_1^{-1}g_2 \in K
            </me>.
            By <xref ref="proposition_Cosets_cosets_theorem_1">Proposition</xref>
            in the Cosets chapter (parts (1) and (2)),
            this implies that <m>g_1K = g_2K</m>.
          </p>
        </li>
        <li>
          <p>
            Onto: Let <m>h</m> be an arbitrary element of <m>f(G)</m>.
            Then there exists <m>g \in G</m> such that <m>f(g)=h</m>.
            By the definition of <m>F</m>,
            we have also that <m>F(gK) = h</m>.
          </p>
        </li>
        <li>
          <p>
            Preserves operations: Using properties of normal subgroups, we have:
            <me>
              F(g_1Kg_2K) = F(g_1g_2K) = f(g_1g_2) = f(g_1)f(g_2) = F(g_1K)F(g_2K)
            </me>.
          </p>
        </li>
      </ul>
    </p>
  </proof>
  <example xml:id="example_Homomorphism_homo_cyclic">
    <statement>
      <p>
        Let <m>G</m> be a cyclic group with generator <m>g</m>.
        Define a map <m>f : {\mathbb Z} \rightarrow G</m> by <m>n \mapsto g^n</m>.
        This map is a surjective homomorphism<idx><h>Homomorphism</h><h>surjective</h></idx> since
        <me>
          f( m + n) = g^{m+n} = g^m g^n = f(m) f(n)
        </me>.
      </p>
      <p>
        Clearly <m>f</m> is onto.
        If <m>|g| = m</m>, then <m>g^m = e</m>.
        Hence, <m>\ker f = m {\mathbb Z}</m> and <m>{\mathbb Z} / \ker f = {\mathbb Z} / m {\mathbb Z} \cong G</m>.
        On the other hand, if the order of <m>g</m> is infinite,
        then <m>\ker f = 0</m> and <m>\phi</m> is an isomorphism of <m>G</m> and <m>{\mathbb Z}</m>.
        Hence, two cyclic groups are isomorphic exactly when they have the same order.
        We may conclude that up to isomorphism,
        the only cyclic groups are
        <m>{\mathbb Z}</m> and <m>{\mathbb Z}_n</m>.
      </p>
    </statement>
  </example>
</section>