<section xml:id="sec_SigmaNotation_Nested">
  <title>Change of variable and  rearrangement of sums<nbsp/><nbsp/></title>
  <figure>
    <video youtubeplaylist="PL2uooHqQ6T7PW5na4EX8rQX2WvBBdM8Qo"/>
  </figure>
  <p>
    Change of variable (a.k.a. substitution) is an extremely powerful technique in mathematics.
    We've used change of variable in previous chapters,
    and most likely you've seen change of variable when doing integrals in calculus.
    Change of variable can also be used to simplify sums
    (in fact, there is a very close relationship between integrals and sums,
    so it's no surprise that the same techniques are useful in both regimes).
  </p>
  <p>
    Consider for example the following sum:
    <me>
      \sum_{i=2}^{7}(i-1)
    </me>
  </p>
  <p>
    If we write this out term by term,
    we get <m>1+2+3+4+5+6</m> which has a very easy representation as a sigma,
    namely <m>\sum_{j=1}^{6}j</m>.
    It follows that
    <me>
      \sum_{i=2}^{7}(i-1) = \sum_{j=1}^{6}j
    </me>.
  </p>
  <p>
    Writing it this way,
    we can see how we got from one some to the other by making the replacement <m>j = i-1</m>.
    We also had to change the limits of the sum accordingly
    (just like you have to change integral limits when you change variable).
  </p>
  <p>
    A similar example is:
    <md>
      <mrow>\frac{1}{8}\sum_{j=5}^{9} 2^{j-2} \amp = \sum_{j=5}^{9} 2^{j-2} \cdot 2^{-3}</mrow>
      <mrow>\amp =\sum_{j=5}^{9} 2^{j-5}</mrow>
    </md>.
  </p>
  <p>
    We may substitute <m>i = j-5</m>.
    Noticing that <m>j=5 \implies i=0</m> and <m>j=9 \implies i=4</m>,
    we obtain
    <me>
      \frac{1}{8}\sum_{j=5}^{9} 2^{j-2} =\sum_{i=0}^4 2^i
    </me>.
  </p>
  <exercise xml:id="exercise_SigmaNotation_sum1">
    <statement>
      <p>
        Take the following sigma notation examples and change the formula and final value so that the starting value becomes 0 and the sum maintains the same value.
        Calculate the value of both the listed sum and the resulting sum to show that the value is the same.
        <ol type="a">
          <li>
            <p>
              <m>\displaystyle{\sum_{i=3}^{7}2i}</m>
            </p>
          </li>
          <li>
            <p>
              <m>\displaystyle{\sum_{j=7}^{21}\cos(j\pi )}</m>
            </p>
          </li>
          <li>
            <p>
              <m>\displaystyle{\sum_{j=20}^{24}(j-20)}</m>
            </p>
          </li>
        </ol>
      </p>
    </statement>
  </exercise>
  <p>
    Breaking up sums and re-indexing can sometimes make things a lot simpler.
    Consider the following example:
    <me>
      S = \sum_{k=1}^{21} \text{ cis }  \left(\frac{2\pi k}{20} \right)
    </me>.
  </p>
  <p>
    Let's break this up into two sums,
    from <m>k = 1</m> to <m>10</m> and from <m>k=11</m> to <m>21</m>:
    <me>
      S = \sum_{k=1}^{10} \text{ cis }  \left(\frac{2\pi k}{20} \right) + \sum_{k=11}^{21} \text{ cis }  \left(\frac{2\pi k}{20} \right)
    </me>.
  </p>
  <p>
    It would be nice to combine these two sums into one.
    But to do this, we need to make the summation limits the same.
    So we'll change variable: <m>j = k-10</m> in the second sum.
    Then the sum from <m>k=11</m> to <m>21</m> becomes a sum from <m>j=1</m> to <m>11</m>:
    <me>
      S = \sum_{k=1}^{10} \text{ cis }  \left(\frac{2\pi k}{20} \right) + \sum_{j=1}^{11} \text{ cis }  \left(\frac{2\pi (j+10)}{20} \right)
    </me>.
  </p>
  <p>
    Now let's massage the sum over <m>j</m> a little bit.
    Using the properties of <m>\text{ cis }</m>,
    the summand can be rewritten:
    <md>
      <mrow>\text{ cis }  \left(\frac{2\pi (j+10)}{20} \right) \amp = \text{ cis }  \left(\frac{2\pi j}{20} + \pi \right)</mrow>
      <mrow>\amp = \text{ cis } \left(\frac{2\pi j}{20} + \pi \right)</mrow>
      <mrow>\amp = \text{ cis } \left(\frac{2\pi j}{20}\right)\text{ cis } (\pi)</mrow>
      <mrow>\amp  = -\text{ cis } \left(\frac{2\pi j}{20}\right)</mrow>
    </md>.
  </p>
  <p>
    Furthermore,
    we don't change anything if we replace the <m>j</m> with <m>k</m>,
    since it's just a sum index anyway.
    Making these substitutions, we have:
    <me>
      S = \sum_{k=1}^{10} \text{ cis }  \left(\frac{2\pi k}{20} \right) + \sum_{k=1}^{11} -\text{ cis }  \left(\frac{2\pi k}{20} \right)
    </me>.
  </p>
  <p>
    Now we can split the 11'th term off from the second sum,
    and combine the two sums from 1 to 10:
    <md>
      <mrow>S \amp = \sum_{k=1}^{10} \text{ cis }  \left(\frac{2\pi k}{20} \right) + \sum_{k=1}^{10} -\text{ cis }  \left(\frac{2\pi k}{20} \right) - \text{ cis }  \left(\frac{2\pi \cdot 11}{20} \right)</mrow>
      <mrow>\amp = \sum_{k=1}^{10} \left(\text{ cis }  \left(\frac{2\pi k}{20} \right) -\text{ cis }  \left(\frac{2\pi k}{20} \right) \right) - \text{ cis }  \left(\frac{2\pi \cdot 11}{20} \right)</mrow>
      <mrow>\amp = \sum_{k=1}^{10} (0) - \text{ cis }  \left(\frac{2\pi \cdot 11}{20} \right)</mrow>
      <mrow>\amp = -\text{ cis }  \left(\frac{2\pi \cdot 11}{20} \right).</mrow>
      <mrow>\amp = \text{ cis }  \left(\frac{\pi }{10} \right)</mrow>
    </md>.
  </p>
  <exercise>
    <statement>
      <p>
        By splitting up the sums and rearranging,
        evaluate the following sums:
        <ol type="a">
          <li>
            <p>
              <m>\sum_{k=1}^{14} \text{ cis } \left(\frac{6\pi k}{7} \right)</m>
            </p>
          </li>
          <li>
            <p>
              <m>\sum_{k=1}^{15} \text{ cis } \left(\frac{6\pi k}{5} \right)</m>
            </p>
          </li>
        </ol>
      </p>
    </statement>
  </exercise>
  <p>
    We've already seen cases where one sigma is inside another,
    when taking the product of two sums.
    Nested sums like this can often be rearranged to obtain useful formulas.
  </p>
  <example>
    <statement>
      <p>
        Consider the product of the sums
        <m>\sum_{i=0}^{2} 3^i</m> and <m>\sum_{j=0}^{2}3^{-j}</m>.
        By the distributive law and additive commutivity we have:
        <md>
          <mrow>\left(\sum_{i=0}^{2} 3^i\right) \left( \sum_{j=0}^{2}3^{-j}\right) \amp = \sum_{i=0}^{2} \left(3^i \left( \sum_{j=0}^{2}3^{-j}\right) \right)</mrow>
          <mrow>\amp = \sum_{i=0}^{2}  \left( \sum_{j=0}^{2}3^{i-j}\right)</mrow>
          <mrow>\amp = \sum_{i=0}^{2}  \sum_{j=0}^{2}3^{i-j}</mrow>
        </md>.
      </p>
      <p>
        This sum has 9 terms,
        where each term corresponds to a pair <m>(i,j)</m> as shown in <xref ref="fig_productOfSums">Figure</xref>.
        These terms can be arranged along diagonal lines
        (as shown in the figure)
        so that all terms on each diagonal have the same value.
        So we can add the terms diagonal-by-diagonal as follows:
        <md>
          <mrow>\sum_{i=0}^{2}  \sum_{j=0}^{2}3^{i-j} \amp = 3^{-2} + 2\cdot 3^{-1} +3 \cdot 3^0 + 2 \cdot 3^{1} + 3^{2}</mrow>
          <mrow>\amp = 1/9 + 2/3 + 3 + 6 + 9</mrow>
          <mrow>\amp = 18\, \frac{5}{9}</mrow>
        </md>.
      </p>
      <figure xml:id="fig_productOfSums">
        <caption>Grid points corresponding to the terms in the sum: <m>\sum_{i=0}^{2}  \sum_{j=0}^{2} 5^{i-j}</m>.</caption>
        <image width="56%" source="images/productOfSums.png"/>
      </figure>
    </statement>
  </example>
  <exercise>
    <statement>
      <p>
        By following the above argument backwards,
        write the following expressions as a product of sums:
        <ol type="a">
          <li>
            <p>
              <me>
                \sum_{n=1}^3 n3^{3-n} + \sum_{n=1}^2 n3^{n-3}
              </me>
            </p>
          </li>
          <li>
            <p>
              <me>
                \sum_{n=1}^{10} n5^{10-n} + \sum_{n=1}^{9} n5^{n-10}
              </me>
            </p>
          </li>
        </ol>
      </p>
    </statement>
  </exercise>
  <p>
    The situation becomes interesting when the sum inside depends on the the index variable of the outside sigma:
    <me>
      \sum_{i=0}^{3}\sum_{j=0}^{i}1
    </me>
  </p>
  <p>
    Unlike previous double sums,
    the inside sum will change depending on what <m>i</m> is.
    When <m>i=0</m> then <m>\sum_{j=0}^{i}1=\sum_{j=0}^{0}1=1</m> so 1 would be the first term in the outside sum.
    When <m>i=1</m> then <m>\sum_{j=0}^{i}1=\sum_{j=0}^{1}1=1+1=2</m> so 2 would be the next term.
    With each successive term,
    the inside sum increases by 1, so the result is <m>1+2+3+4 = 10</m>.
  </p>
  <p>
    Note that the index of the outer sum may appear in any or all parts of the inner sum.
    Here are some examples:
    <me>
      \sum_{i=0}^{3} \sum_{j=i}^{10}1; \qquad \sum_{i=0}^{3} \sum_{j=1}^{10i}i ; \qquad \sum_{i=0}^{3}\sum_{j=i}^{2i}(3i+x^j)
    </me>.
  </p>
  <p>
    In some cases,
    nested sums may be simplified by exchanging the order of summation.
    Take for example:
    <me>
      \sum_{i=0}^{2}  \sum_{j=0}^{i}1
    </me>
  </p>
  <p>
    The first term has <m>i=0</m> and <m>j=0</m>:
    we write this as <m>(i,j)=(0,0)</m>.
    When <m>i=1</m>, then we have two terms:
    <m>j=0</m> and <m>j=1</m>.
    Finally, when <m>i=2</m>, we have <m>j=0,1</m>, or 2.
    Altogether we have the index pairs:
    <m>(0,0), (1,0), (1,1), (2,0), (2,1), (2,2)</m>.
    These index pairs may be displayed on a grid,
    as shown in <xref ref="fig_summation1">Figure</xref>.
  </p>
  <figure xml:id="fig_summation1">
    <caption>Grid points corresponding to the terms in the sum: <m>\sum_{i=0}^{2}  \sum_{j=0}^{i}1</m>.</caption>
    <image width="56%" source="images/i02j0igraph.png"/>
  </figure>
  <p>
    Alternatively,
    we can arrange these index pairs by <m>j</m> coordinate.
    When <m>j</m> is 0, <m>i</m> takes the values (0,1,2);
    when <m>j</m> is 1, <m>i</m> takes the values of (1,2);
    and when <m>j</m> is 2, <m>i</m> takes the value 2.
    This can be expressed as the sum:
    <me>
      \sum_{j=0}^{2} \sum_{i=j}^{2}1
    </me>
  </p>
  <p>
    So far our examples have only two sigmas,
    but it's quite possible to have an unlimited number of nested sigmas.
    For example,
    with three nested sigmas we would have grid points in three dimensions.
    It doesn't matter what order you sum the terms in<ndash/>as long as you include them all!
  </p>
  <exercise xml:id="exercise_SigmaNotation_nested1">
    <statement>
      <p>
        Draw a grid point diagram
        (similar to <xref ref="fig_summation1">Figure</xref>)
        for each of the following sums.
        Then use the grid point diagram as a guide to exchanging the order of summation.
        <ol type="a">
          <li>
            <p>
              <m>\displaystyle{\sum_{i=0}^{4}\sum_{j=0}^{8}i}</m>
            </p>
          </li>
          <li>
            <p>
              <m>\displaystyle{\sum_{j=0}^{3} \sum_{i=j}^{j+3} (i+j)}</m><nbsp/><nbsp/><nbsp/><nbsp/>(Write as the sum of two summations.)
            </p>
          </li>
          <li>
            <p>
              <m>\displaystyle{\sum_{k=0}^{7}\sum_{i=0}^{k}(2i+1) }</m>
            </p>
          </li>
          <li>
            <p>
              <m>\displaystyle{\sum_{i=1}^{6}\sum_{j=i}^{i+1} (i-j) }</m><nbsp/><nbsp/><nbsp/><nbsp/>(Write as a nested sum plus two additional terms.)
            </p>
          </li>
          <li>
            <p>
              <m>\displaystyle{\sum_{i=1}^{5}\sum_{j=i}^{10} ij }</m>
            </p>
          </li>
          <li>
            <p>
              <m>\displaystyle{\sum_{i=m}^{n}\sum_{j=i}^{2n}jx^i }</m><nbsp/><nbsp/><nbsp/><nbsp/>(Write as the sum of two summations.)
            </p>
          </li>
          <li>
            <p>
              <m>\displaystyle{\sum_{i=m}^{n}\sum_{j=0}^{i}(i-j)^2 }</m><nbsp/><nbsp/><nbsp/><nbsp/>(You may assume <m>m>0</m>.
              Write as the sum of two summations.)
            </p>
          </li>
        </ol>
      </p>
    </statement>
  </exercise>
  <exercise xml:id="exercise_SigmaNotation_interchangeSum">
    <statement>
      <ol type="a">
        <li>
          <p>
            Using a grid point diagram,
            interchange the order of summation in the following nested sum:
            <me>
              \sum_{k=1}^{5} \sum_{\ell=1}^k (\ell + k)
            </me>
          </p>
        </li>
        <li>
          <p>
            Using a grid point diagram,
            interchange the order of summation in the following nested sum:
            <me>
              \sum_{i=1}^{7} \sum_{j=1}^i ij
            </me>
          </p>
        </li>
        <li>
          <p>
            Using what you've from (a) and (b) above,
            give a general formula for intechanging sums of the form:
            <me>
              \sum_{m=1}^M \sum_{n=1}^m f(m,n)
            </me>,
            where <m>f(m,n)</m> is an arbitrary expression involving the variables <m>m</m> and <m>n</m>.
          </p>
        </li>
      </ol>
    </statement>
  </exercise>
  <exercise>
    <statement>
      <ol type="a">
        <li>
          <p>
            In <xref ref="exercise_SigmaNotation_interchangeSum">Exercise</xref>,
            all sums had 1 as lower limit.
            Repeat the exercise
            (parts a,b,c)
            but use 0 as the lower limit on all sums.
          </p>
        </li>
        <li>
          <p>
            Repeat <xref ref="exercise_SigmaNotation_interchangeSum">Exercise</xref> again,
            but use 2 as the lower limit on all sums.
          </p>
        </li>
        <li>
          <p>
            Based on what you have learned from (a) and (b),
            give a general formula for interchanging the order of summation in the following expression:
            <me>
              \sum_{m=a}^b \sum_{n=a}^m f(m,n)
            </me>,
          </p>
        </li>
      </ol>
    </statement>
  </exercise>
  <exercise xml:id="exercise_SigmaNotation_nested2">
    <statement>
      <p>
        Using exchange of summation and other sum manipulation techniques,
        find the exact values of the following sums:
        <ol type="a">
          <li>
            <p>
              <m>\displaystyle{\sum_{i=1}^{9} \sum_{j=1}^{7} i(8-j)}</m>
            </p>
          </li>
          <li>
            <p>
              <m>\displaystyle{\sum_{i=1}^{10} \sum_{j=1}^{10} (j-i)}</m>
            </p>
          </li>
          <li>
            <p>
              <m>\displaystyle{\sum_{i=1}^{10} \sum_{j=1}^i \frac{1}{11-j}}</m>
            </p>
          </li>
          <li>
            <p>
              <m>\displaystyle{\sum_{i=1}^{10} \sum_{j=i}^{10} \frac{i}{j(j+1)}}</m>
            </p>
          </li>
          <li>
            <p>
              <m>\displaystyle{\sum_{i=1}^{20} \sum_{j=1}^i \frac{i}{(400-j^2)+j+20}}</m> (*Hint*)
            </p>
          </li>
          <li>
            <p>
              <m>\displaystyle{\sum_{i=1}^{10} \sum_{j=1}^i (j+i)}</m>
            </p>
          </li>
        </ol>
      </p>
    </statement>
  </exercise>
</section>