<section xml:id="sec_Polynomials_PropertiesAndSigmaNotation">
  <title>Polynomial properties and summation notation</title>
  <p>
    In the past several sections,
    we have looked at polynomials with different types of coefficients.
    These different types of polynomials have a lot in common.
    In this section,
    we will look more deeply into just what it is that is common to all.
  </p>
  <p>
    Since we want our discussion to be general,
    we don't want to restrict ourselves to any particular set of coefficients.
    Instead, we will denote our polynomials by <m>R[x]</m>,
    where the set of coefficients <m>R</m> can represent <m>{\mathbb R},{\mathbb C},{\mathbb Q},{\mathbb Z},{\mathbb Z}_n</m>,
    or <m>{\mathbb M}_n</m> (i.e.
    <m>n \times n</m> matrices).
    This means that the results of this section will be valid for many different types of polynomials.
    The only properties that we require of the set <m>R</m> are the following:
    <ol type="I">
      <li>
        <p>
          <m>R</m> has two binary operations,
          denoted as + and <m>\cdot</m> (i.e. addition and multiplication);
        </p>
      </li>
      <li>
        <p>
          <m>R</m> is closed under both addition and multiplication;
        </p>
      </li>
      <li>
        <p>
          Addition in <m>R</m> is commutative;
        </p>
      </li>
      <li>
        <p>
          Addition and multiplication are both associative;
        </p>
      </li>
      <li>
        <p>
          Multiplication distributes over addition: e.g.
          <m>a \cdot (b+c) = a\cdot b + a\cdot c</m> and <m>(a+b) \cdot c = a \cdot c + b \cdot c</m>.
        </p>
      </li>
    </ol>
  </p>
  <p>
    (We will see somewhat later that all of these properties a characteristic of a type of mathematical structure called a
    <q>ring</q>. But for the time being,
    we may simply recognize them as properties that are common to the number systems that we have been using so far.)
  </p>
  <p>
    Given that <m>R</m> has addition and multiplication operations,
    we may define addition and multiplication in <m>R[x]</m> using <xref ref="definition_Polynomials_defsumpoly">Definitions</xref>
    and <xref ref="definition_Polynomials_defprodpoly"></xref>.
    Let's first make sure that the definitions give well-behaved,
    closed operations in <m>R[x]</m>.
  </p>
  <proposition xml:id="proposition_Polynomials_polyclosed">
    <statement>
      <p>
        Given that <m>R</m> satisfies conditions (I)-(V) listed above.
        Then <xref ref="definition_Polynomials_defsumpoly">Definitions</xref>
        and <xref ref="definition_Polynomials_defprodpoly"></xref>
        produce closed addition and multiplication operations in <m>R[x]</m>.
      </p>
    </statement>
  </proposition>
  <p>
    You will prove <xref ref="proposition_Polynomials_polyclosed">Proposition</xref> in the following exercise.
  </p>
  <exercise>
    <statement>
      <ol type="a">
        <li>
          <p>
            Prove that <xref ref="definition_Polynomials_defsumpoly">Definition</xref>
            gives a closed operation in <m>R[x]</m> by showing that whenever <m>p(x)</m> and <m>q(x)</m> are polynomials in <m>R[x]</m>,
            then <m>p(x)+q(x)</m> is also a polynomial in <m>R[x]</m>.
          </p>
        </li>
        <li>
          <p>
            Prove that <xref ref="definition_Polynomials_defprodpoly">Definition</xref>
            gives a closed multiplication operation in <m>R[x]</m> by showing that whenever <m>p(x)</m> and <m>q(x)</m> are polynomials in <m>R[x]</m>,
            then <m>p(x)q(x)</m> is also in <m>R[x]</m>.
          </p>
        </li>
      </ol>
    </statement>
  </exercise>
  <p>
    Now that we've shown that the operations of addition and multiplication in <m>R[x]</m> are properly defined,
    we may verify that these operations have workable properties.
  </p>
  <proposition xml:id="proposition_Polynomials_polysumcommuteassociate">
    <statement>
      <p>
        Given that <m>R</m> satisfies conditions (I)-(V) listed above,
        then addition in <m>R[x]</m> is both commutative:
        <me>
          p(x)+q(x) = q(x) + p(x)
        </me>,
        and associative:
        <me>
          (p(x) + q(x)) + r(x)  = p(x) + (q(x) + r(x))
        </me>.
      </p>
    </statement>
  </proposition>
  <proof>
    <p>
      First, we show commutativity: Given two polynomials <m>p(x)</m> and <m>q(x)</m> where
      <md>
        <mrow>p(x)  = \sum^{m}_{i=0} a_i x^i; \qquad q(x)  = \sum^{n}_{i=0} b_i x^i</mrow>
      </md>,
      then
      <me>
        p(x) + q(x) =  \sum_{i=0}^{\max(m,n)} (a_i + b_i) x^i
      </me>,
      and
      <me>
        p(x) + q(x) =  \sum_{i=0}^{\max(m,n)} (b_i + a_i) x^i
      </me>.
    </p>
    <p>
      Since the addition is commutative,
      we have <m>a_i + b_i = b_i + a_i</m> for all <m>i</m>.
      It follows that all coefficients of
      <m>p(x) + q(x)</m> are equal to the corresponding coefficients of <m>q(x) + p(x)</m>.
      By the definition of polynomial equality,
      this means that <m>p(x) + q(x) = q(x) + p(x)</m>.
    </p>
  </proof>
  <proof>
    <p>
      Next we'll prove additive associativity.
      To do this, we must introduce a third polynomial, <m>r(x)</m>,
      with degree <m>\ell</m> and coefficients <m>c_i, i=0 \ldots \ell</m>.
      <me>
        r(x) = \sum^{\ell}_{i=0} c_ix^i
      </me>.
    </p>
    <p>
      We have,
      <md>
        <mrow>(p(x)+q(x))+r(x) =\amp  \bigg(\sum^{m}_{i=0} a_i x^i+\sum^{n}_{i=0} b_i x^i \bigg)+  \sum^{\ell}_{i=0} c_ix^i</mrow>
        <mrow>=\amp  \bigg(\sum_{i=0}^{\max(m,n)} (a_i + b_i) x^i\bigg)+  \sum^{\ell}_{i=0} c_ix^i</mrow>
        <mrow>=\amp  \sum_{i=0}^{\max((m,n),\ell)} (a_i + b_i+c_i) x^i</mrow>
        <mrow>=\amp  \sum_{i=0}^{\max(m,(n,\ell))} (a_i + b_i+c_i) x^i</mrow>
        <mrow>=\amp  \sum^{m}_{i=0} a_i x^i+\sum_{i=0}^{\max(n,\ell)} (b_i + c_i) x^i</mrow>
        <mrow>=\amp  \sum^{m}_{i=0} a_i x^i+\bigg(\sum^{n}_{i=0} b_i x^i+\sum^{\ell}_{i=0} c_i x^i \bigg)</mrow>
        <mrow>=\amp  p(x)+(q(x)+r(x))</mrow>
      </md>.
    </p>
    <p>
      Therefore, by the definition of polynomial equality and polynomial addition,
      <m>(p(x)+q(x))+r(x)=p(x)+(q(x)+r(x))</m>.
      Note that we have used additive associativity of the coefficients (i. e.
      <m>(a_i+b_i)+c_i=a_i+(b_i+c_i)</m> for all <m>i</m>).
    </p>
  </proof>
  <p>
    It's also true that the set <m>R[x]</m> has an additive identity and additive inverses.
    We'll look first at identity.
  </p>
  <proposition xml:id="proposition_Polynomials_polyadditiveidentity">
    <statement>
      <p>
        Given that <m>R</m> satisfies properties (I)-(V), then the additive identity of <m>R[x]</m> is <m>0x^0</m>,
        where <m>0</m> denotes the additive identity of <m>R</m>.
      </p>
    </statement>
  </proposition>
  <proof>
    <p>
      The proof has two parts: (i)
      <m>p(x)+0x^0=p(x)</m> and (ii) <m>0x^0+p(x)=p(x), \forall p(x) \in R[x]</m>.
      We'll prove (i) and leave (ii) as an exercise.
    </p>
    <p>
      (i) Given an arbitrary polynomial <m>p(x)= \sum^{m}_{i=0} a_i x^i \in R[x]</m>.
      Then,
      <md>
        <mrow>p(x)+0x^0=\amp \left(\sum^{m}_{i=0} a_i x^i\right)+0x^0</mrow>
        <mrow>=\amp \sum^{m}_{i=0} (a_i+0) x^i</mrow>
        <mrow>=\amp \sum^{m}_{i=0} a_i x^i</mrow>
        <mrow>=\amp p(x)</mrow>
      </md>
    </p>
    <p>
      So part (i) of the proof is finished.
    </p>
    <exercise>
      <statement>
        <p>
          Complete part (ii) of the proof of Proposition 1.6.6.
        </p>
      </statement>
    </exercise>
  </proof>
  <p>
    In the following we'll write the additive identity of <m>R[x]</m> as <m>0</m> instead of <m>0x^0</m>,
    but don't forget that the additive identity of <m>R[x]</m> is also a polynomial in <m>R[x]</m>.
  </p>
  <p>
    Before we prove additive inverse,
    we should first clarify some notation.
    If <m>a</m> is an element of a ring <m>R</m>,
    then we'll write the additive inverse of <m>a</m> as <m>-a</m>.
    (This is obvious if <m>R</m> is <m>\mathbb{R}</m>, <m>\mathbb{Z}</m>,
    or some other familiar set of numbers<ndash/>but we also need to think about the general case where <m>R</m> is some other set such as <m>\mathbb{Z}_n</m>,
    and the <m>+</m> operation is not regular addition.)
    Using this notation,
    we may now characterize the additive inverse of a polynomial.
  </p>
  <exercise>
    <statement>
      <p>
        Determine the additive inverse of each element in <m>Z_5</m> and explain your answer.
      </p>
    </statement>
  </exercise>
  <proposition xml:id="proposition_Polynomials_polyadditiveinverse">
    <statement>
      <p>
        Let <m>p(x)=\sum_{i=0}^n a_i x^i</m> be a polynomial in <m>R[x]</m>,
        where <m>R</m> satisfies properties (I)-(V).
        Then the additive inverse of <m>p(x)</m> is <m>q(x)=\sum_{i=0}^n (-a_i) x^i</m>,
        where <m>-a_i</m> is the additive inverse of <m>a_i</m> in <m>R</m>.
      </p>
    </statement>
  </proposition>
  <exercise>
    <statement>
      <p>
        Prove <xref ref="proposition_Polynomials_polyadditiveinverse">Proposition</xref>
        by showing that <m>p(x) + q(x)</m> and
        <m>q(x)+ p(x)</m> both sum to the additive identity of <m>R[x]</m>.
      </p>
    </statement>
  </exercise>
  <p>
    If we compare our results with the definition of group (<xref ref="definition_ModularArithmetic_group">Definition</xref>,
    we make an important discovery:
  </p>
  <proposition xml:id="proposition_Polynomials_polyadditivegroup">
    <statement>
      <p>
        Let <m>R[x]</m> be the set of polynomials over a set <m>R</m> that satisfies properties (I)-(V).
        Then <m>R[x]</m> is an abelian group under addition
        (recall that
        <q>abelian</q>
        means that the group's operation is commutative).
      </p>
    </statement>
  </proposition>
  <exercise>
    <statement>
      <p>
        Prove <xref ref="proposition_Polynomials_polyadditivegroup">Proposition</xref>.
        You may use the propositions that we already proved in this section.
      </p>
    </statement>
  </exercise>
  <p>
    Next, we consider the proof for multiplicative associativity in general,
    but before giving a proof, let's do an example to see how this works.
  </p>
  <exercise xml:id="exercise_Polynomials_poly5">
    <statement>
      <p>
        Show that the multiplication of two linear polynomials and one quadratic polynomial is associative. (use
        <m>a_0+a_1x,
        b_0+b_1x</m>, and <m>c_0+c_1x+c_2x^2</m> as your polynomials.)
      </p>
    </statement>
  </exercise>
  <p>
    We've been talking about polynomial addition<mdash/>now it's multiplication's turn.
    First we prove multiplicative associativity in <m>R[x]</m>:
  </p>
  <proposition xml:id="proposition_Polynomials_polymultassociate">
    <statement>
      <p>
        Multiplication in <m>R[x]</m> is associative:
        <me>
          (p(x) q(x)) r(x)  = p(x) (q(x) r(x))
        </me>.
      </p>
    </statement>
  </proposition>
  <proof>
    <p>
      We've seen that the product of two polynomials <m>p(x)</m> and <m>q(x)</m> may be written in summation notation as:
      <me>
        p(x) q(x) =\sum_{i=0}^{m}\sum_{j=0}^{n}a_i b_j x^{i+j}
      </me>
    </p>
    <p>
      Now we multiply a third polynomial,
      <m>r(x)</m>, to calculate its product with <m>(p(x)q(x))</m>:
      <md>
        <mrow>(p(x) q(x))r(x) =\amp   \Big( \sum_{i=0}^{m}\sum_{j=0}^{n}a_i b_j x^{i+j} \Big)\Big(\sum_{k=0}^{\ell} c_k x^k \Big)</mrow>
        <mrow>=\amp    \sum_{i=0}^{m}\sum_{j=0}^{n} \Big(a_i b_j x^{i+j}\Big(\sum_{k=0}^{\ell} c_k x^k \Big) \Big)</mrow>
        <mrow>=\amp  \sum_{i=0}^{m}\sum_{j=0}^{n}\sum_{k=0}^{\ell} a_i b_j x^{i+j} \cdot c_k x^k</mrow>
        <mrow>=\amp   \sum_{i=0}^{m}\sum_{j=0}^{n}\sum_{k=0}^{\ell} a_i b_j  c_k x^{i+j+k}</mrow>
      </md>.
    </p>
    <p>
      In the above calculation we have twice brought multiplicative terms inside of summations,
      using the distributive law.
      The last step uses a familiar exponent rule.
    </p>
    <p>
      To complete the proof of associativity,
      we need to show that the summation expression for
      <m>p(x) (q(x)r(x))</m> may be simplified into the same expression.
      The calculation is very similar,
      and we leave it as an exercise:
    </p>
    <exercise>
      <statement>
        <p>
          Show <m>p(x) (q(x)r(x))</m> also simplifies to <m>\displaystyle{\sum_{i=0}^{m}\sum_{j=0}^{n}\sum_{k=0}^{\ell} a_i b_j c_k x^{i+j+k}}</m>.
          Give a justification for each step of your calculation.
        </p>
      </statement>
    </exercise>
    <p>
      The exercise shows that <m>(p(x) q(x)) r(x)</m> and
      <m>p(x) (q(x) r(x))</m> both simplify to the same expression,
      so they are equal.
      This completes the proof.
    </p>
  </proof>
  <p>
    Next we consider the distributive property for polynomials.
  </p>
  <proposition xml:id="proposition_Polynomials_polyleftrightdistributivity">
    <statement>
      <p>
        Polynomials in <m>R[x]</m> have both right distributivity across addition:
        <me>
          (q(x)+r(x)) p(x) = q(x)p(x)+r(x)p(x)
        </me>,
        and left distributivity across addition:
        <me>
          p(x)(q(x)+r(x)) = p(x)q(x)+p(x)r(x)
        </me>.
      </p>
    </statement>
  </proposition>
  <proof>
    <p>
      To show right distributivity, we have:
      <md>
        <mrow>(q(x)+r(x)) p(x)=\amp \bigg(\sum^{n}_{j=0} b_j x^j +  \sum^{\ell}_{j=0} c_jx^j\bigg)\sum^{m}_{i=0} a_i x^i</mrow>
        <mrow>=\amp \bigg(\sum_{j=0}^{\max(n,\ell)} (b_j + c_j) x^j\bigg)\sum^{m}_{i=0} a_i x^i</mrow>
        <mrow>=\amp \bigg(\sum_{j=0}^{\max(n,\ell)} (b_j x^j+ c_j x^j)\bigg)\sum^{m}_{i=0}a_ix^i</mrow>
        <mrow>=\amp \sum_{j=0}^{\max(n,\ell)}\bigg((b_j x^j+ c_j x^j)\sum^{m}_{i=0}a_ix^i\bigg)</mrow>
        <mrow>=\amp \sum_{j=0}^{\max(n,\ell)}\sum^{m}_{i=0} (b_j x^j+ c_j x^j)a_ix^i</mrow>
        <mrow>=\amp \sum_{j=0}^{\max(n,\ell)}\sum^{m}_{i=0} (b_j x^ja_ix^i+ c_j x^ja_ix^i)</mrow>
        <mrow>=\amp \sum_{j=0}^{\max(n,\ell)}\sum^{m}_{i=0} b_j x^ja_ix^i+ \sum_{j=0}^{\max(n,\ell)}\sum^{m}_{i=0}c_j x^ja_ix^i</mrow>
        <mrow>=\amp \sum_{j=0}^{n}\sum^{m}_{i=0} b_j x^ja_ix^i+ \sum_{j=0}^{\ell}\sum^{m}_{i=0}c_j x^ja_ix^i</mrow>
        <mrow>=\amp \sum^{n}_{j=0} b_j x^j\sum^{m}_{i=0} a_i x^i+ \sum^{\ell}_{j=0} c_jx^j \sum^{m}_{i=0} a_i x^i</mrow>
        <mrow>=\amp q(x)p(x)+r(x)p(x)</mrow>
      </md>,
      which gives us right distributivity.
      We'll leave left distributivity up to you:
    </p>
    <exercise>
      <statement>
        <p>
          Provide justification for each of the steps in the calculation in <xref ref="proposition_Polynomials_polyleftrightdistributivity">Proposition</xref>
        </p>
      </statement>
    </exercise>
    <exercise>
      <statement>
        <p>
          Prove that polynomials in <m>R[x]</m> have left distributivity across addition.
        </p>
      </statement>
    </exercise>
  </proof>
</section>