<section xml:id="sec_Induction_BasicInduction">
  <title>Basic examples of induction proofs</title>
  <p>
    Below is a complete proof of the formula for the sum of the first <m>n</m> integers,
    that can serve as a model for proofs of similar sum/product formulas.<fn>
    This section was taken
    (with permission!)
    from A. J. Hildebrand's excellent notes on induction
    (reformatted and minor edits by C.T.).
    </fn>
  </p>
  <proposition xml:id="proposition_Induction_Induction1">
    <statement>
      <p>
        For all <m>n\in\NN</m>,
        the following equation (which we denote as <m>P(n)</m>) is true:
        <me>
          \sum_{i=1}^n i=\frac{n(n+1)}{2}. \tag{\(P(n)\)}
        </me>
      </p>
    </statement>
  </proposition>
  <proof>
    <p>
      <em>(By induction)</em>:
    </p>
    <p>
      <em>Base case:</em> When <m>n=1</m>,
      the left side of <m>P(n)</m> is <m>1</m>,
      and the right side is <m>1(1+1)/2=1</m>,
      so both sides are equal and <m>P(n)</m> holds for <m>n=1</m>.
    </p>
    <p>
      <em>Induction step:</em> Let <m>k\in\NN</m> be given and suppose formula <m>P(n)</m> holds for <m>n=k</m>.
      Then
      <md>
        <mrow>\sum_{i=1}^{k+1}i\amp =\sum_{i=1}^k i + (k+1)\text{ (by definition of \(\sum\) notation) }</mrow>
        <mrow>\amp =\frac{k(k+1)}{2}+(k+1) \text{ (by induction hypothesis) }</mrow>
        <mrow>\amp =\frac{k(k+1)+2(k+1)}{2} \text{ (by algebra) }</mrow>
        <mrow>\amp =\frac{(k+1)((k+1)+1)}{2} \text{ (by algebra) } </mrow>
      </md>.
    </p>
    <p>
      Thus, <m>P(n)</m> holds for <m>n=k+1</m>,
      and the proof of the induction step is complete.
    </p>
    <p>
      <em>Conclusion:</em> By the principle of induction,
      we have proved that <m>P(n)</m> holds for all <m>n\in\NN</m>.
    </p>
  </proof>
</section>