<section xml:id="sec_Polynomials_OperationsAndSigmaNotation">
  <title>Polynomial operations in summation notation</title>
  <p>
    In the preceding section, we discussed familiar polynomial operations.
    In this section we give general formulas for these operations in terms of summation notation.
    These formulas are important both theoretically and practically:
    theoretically,
    because they give us a way to express general polynomial operations in proofs;
    and practically,
    because they provide instructions for programming polynomial operations on computers.
  </p>
  <p>
    So far we have been using polynomials with real
    (and occasionally complex)
    coefficients<ndash/>but keep in mind that the formulas that we obtain will also apply to other types of polynomials as well,
    as we shall see in <xref ref="sec_Polynomials_ExoticPolynomials">Section</xref>.
  </p>
  <p>
    First we give the summation representation for an arbitrary polynomial:
  </p>
  <definition>
    <statement>
      <p>
        {sumPoly} A polynomial may be written as
        <me>
          f(x) = a_0 + a_1 x +a_2 x^2 + \cdots + a_N x^N = \sum^{N}_{n=0} a_n x^n
        </me>,
      </p>
      <p>
        Where <m>a_n</m> is the <term>coefficient</term>
            <idx><h>Polynomial</h><h>coefficients</h></idx>
        of <m>x^n</m>,
        <m>n=1,2, \ldots N</m>.
        It is possible for <m>a_n = 0</m>,
        in which case we usually omit the corresponding <m>x^n</m> term
        (for instance,
        we write <m>-7 + x^2</m> rather than <m>-7 + 0x + x^2</m>).
        When we write a polynomial as a sum in this way we will <term>assume</term>
        that <m>a_N \neq 0</m> (here <m>a_N</m> is called the
        <term>leading coefficient</term>.
            <idx><h>Polynomial</h><h>leading coefficient</h></idx>
        Thus the largest power of <m>x</m> that appears in the polynomial is <m>x^N</m>:
        this largest power is called the
        <term>degree</term><idx><h>Degree</h><h>of a polynomial</h></idx> of the polynomial.
      </p>
    </statement>
  </definition>
  <remark>
    <p>
      According to <xref ref="definition_Polynomials_sumPoly">Definition</xref>,
      we write polynomials in ascending order.
      This differs from <xref ref="sec_Polynomials_PolynomialArithmetic">Section</xref>,
      where we wrote polynomials in descending order as is customary in secondary school.
      Since the operation <sq>+</sq> is commutative,
      the two ways are equivalent:
      but we will increasingly use this new way,
      which turns out to be useful for a number of reasons.
    </p>
  </remark>
  <example xml:id="example_Polynomials_poly3_5">
    <statement>
      <p>
        Express the following polynomials in summation notation:
        <ol type="a">
          <li>
            <p>
              <m>p_1(x)=1 + x+x^2+x^3</m>
            </p>
          </li>
          <li>
            <p>
              <m>p_2(x)=0 + x+2x^2+3x^3+4x^4+5x^5+6x^6+7x^7</m>
            </p>
          </li>
          <li>
            <p>
              <m>p_3(x)=5 x+4x^2+3x^3+2x^4</m>
            </p>
          </li>
          <li>
            <p>
              <m>p_4(x)=x+4x^2+9x^3+16x^4+25x^5</m>
            </p>
          </li>
          <li>
            <p>
              <m>p_5(x)=-3ix^3+4x^4+5i^5x^5</m> (note that here <m>i</m> denotes <m>\sqrt{-1}</m>)
            </p>
          </li>
          <li>
            <p>
              <m>p_6(x)=\sqrt{2}\cis(\pi/3)x^3+\sqrt{3}\cis(2\pi/3)x^6-x^9 + 2\cis(4\pi/3)x^{12} + \sqrt{5}\cis(5\pi/3)x^{15} + \sqrt{6}x^{18}</m>
            </p>
          </li>
          <li>
            <p>
              <m>p_7(x)=0+\frac{1}{2}x+\frac{2}{3}x^2+\frac{3}{4}x^3+\frac{4}{5}x^4</m>
            </p>
          </li>
          <li>
            <p>
              <m>p_8(x)=i+(1+2i)x+(2+3i)x^2+(3+4i)x^3+(4+5i)x^4+(5+6i)x^5+(6+7i)x^6</m>
            </p>
          </li>
        </ol>
      </p>
      <p>
        {Answers:}
        <ol type="a">
          <li>
            <p>
              <m>p_1(x) = \sum_{j=0}^{3} x^j</m>
            </p>
          </li>
          <li>
            <p>
              <m>p_2(x)=\sum_{m=0}^{7} mx^m</m>
            </p>
          </li>
          <li>
            <p>
              <m>p_3(x)=\sum_{k=1}^{4} (6-k)x^k</m>
            </p>
          </li>
          <li>
            <p>
              <m>p_4(x)=\sum_{\ell=0}^{5} \ell^2x^\ell</m>
            </p>
          </li>
          <li>
            <p>
              <m>p_5(x) = \sum_{n=3}^{5}ni^nx^n</m>
            </p>
          </li>
          <li>
            <p>
              <m>p_6(x) = \sum_{q=1}^{6}\sqrt{q+1}\cis(q\pi/3)x^{3q}</m>
            </p>
          </li>
          <li>
            <p>
              <m>p_7(x) = \sum_{i=0}^{5}\frac{ix^i}{i+1}</m>
            </p>
          </li>
          <li>
            <p>
              <m>p_8(x) = \sum_{a=0}^{6}(a+(a+1)i)x^a</m>
            </p>
          </li>
        </ol>
      </p>
      <p>
        Note that we don't always begin the sum at 0, depending on the polynomial.
        Also, the power of <m>x</m> may be a function of the index,
        as in <m>p_6</m>.
      </p>
    </statement>
  </example>
  <exercise xml:id="exercise_Polynomials_poly3l">
    <statement>
      <p>
        Write down the polynomial that each summation represents.
        <ol type="a">
          <li>
            <p>
              <m>p(x) = \sum_{j=0}^{6}( j^2+2)x^{3j}</m>
            </p>
          </li>
          <li>
            <p>
              <m>p(x) = \sum_{r=2}^{5} (r+1)i^rx^r</m>
            </p>
          </li>
          <li>
            <p>
              <m>p(x) = \sum_{s=0}^{8} (-1)^sx^{2s}</m>
            </p>
          </li>
        </ol>
      </p>
    </statement>
  </exercise>
  <exercise xml:id="exercise_Polynomials_poly4">
    <statement>
      <p>
        Re-express the following polynomials in summation notation,
        and give the degree of each polynomial.
        <ol type="a">
          <li>
            <p>
              <m>2 + 0x + 6x^2 + 0x^3 + 10x^4 + 0x^5 + 14x^6 +0x^7 + 18x^8</m>
            </p>
          </li>
          <li>
            <p>
              <m>\cis(\frac{\pi}{2})x^2 + 0x^3 + \cis(\pi)x^4 + 0x^5 + \cis(\frac{3\pi}{2})x^6</m>
            </p>
          </li>
          <li>
            <p>
              <m>1+ 2x + 4x^2 + 8x^3 + 16x^4 + 32x^5</m>
            </p>
          </li>
          <li>
            <p>
              <m>1+4x+11x^2+30x^3+85x^4</m> (*Hint*)
            </p>
          </li>
          <li>
            <p>
              <m>1-\frac{1}{3}x + \frac{1}{5}x^2 - \frac{1}{7}x^3 + \frac{1}{9}x^4 - \frac{1}{11}x^5</m>
            </p>
          </li>
        </ol>
      </p>
    </statement>
  </exercise>
  <remark>
    <p>
      In cases where there is no apparent pattern in the coefficients,
      then summation notation may not be beneficial.
      For example, suppose:
      <me>
        p(x) = 7+ 22x^2 + x^3-6x^6+4x^8-x^9
      </me>.
    </p>
    <p>
      Since there's no clear pattern in the coefficients,
      there's no advantage in writing <m>p(x)</m> in summation notation.
    </p>
  </remark>
  <p>
    Although the following definition may seem rather obvious,
    nonetheless we should state it to be precise.
  </p>
  <definition>
    <statement>
      <p>
        {PolynomialEquality} Two polynomials are said to be
        <term>equal</term><idx><h>Equality</h><h>of polynomials</h></idx> if and only if their corresponding coefficients are equal.
        That is, if we let
        <me>
          p(x)  = \sum^{M}_{m=0} a_m x^m; \qquad q(x)  = \sum^{N}_{n=0} b_n x^n
        </me>,
        then <m>p(x) = q(x)</m> if and only if <m>M=N</m> and
        <m>a_m = b_m</m> for all <m>0 \leq m \leq M</m>.
      </p>
    </statement>
  </definition>
  <p>
    Now we're ready to express our arithmetical rules in summation notation.
  </p>
  <definition>
    <statement>
      <p>
        {defsumpoly} We define the <em>sum of two polynomials</em><idx><h>Sum</h><h>of polynomials</h></idx>
            <idx><h>Polynomials</h><h>sum</h></idx>
        as follows.
        Let
        <md>
          <mrow>p(x)  = \sum^{M}_{m=0} a_m x^m ; \qquad q(x)  = \sum^{N}_{n=0} b_n x^n</mrow>
        </md>,
      </p>
      <p>
        Then the sum of <m>p(x)</m> and <m>q(x)</m> is
        <me>
          p(x) + q(x) =  \sum_{k=0}^{\max(M,N)} (a_k + b_k) x^k
        </me>.
      </p>
      <p>
        In this formula,
        if <m>M>N</m> then it's understood that <m>b_k=0</m> when <m>k>N</m>;
        and if <m>N>M</m> then it's understood that <m>a_k = 0</m> when <m>k>M</m>.
      </p>
    </statement>
  </definition>
  <p>
    Notice that we have taken the upper limit of the sum to
    <m>\max(M,N)</m> in order to make sure to include all nonzero terms from both polynomials.
  </p>
  <p>
    Now that we have a formula for adding polynomials,
    the next step is to obtain a formula for multiplying polynomials,
    using summation notation.
    To do this, let's repeat the polynomial multiplication procedure we used in <xref ref="sec_Polynomials_PolynomialArithmetic">Section</xref>,
    only this time we'll use two general polynomials instead of specific examples.
    As with addition, we use
    <me>
      p(x)  = \sum^{M}_{m=0} a_m x^m; \qquad q(x)  = \sum^{N}_{n=0} b_n x^n
    </me>.
  </p>
  <p>
    In the multiplication example in <xref ref="sec_Polynomials_PolynomialArithmetic">Section</xref>,
    we split up the first polynomial,
    and multiplied each term of the first polynomial by the second polynomial.
    When applied to <m>p(x)</m> and <m>q(x)</m>, this becomes:
    <md>
      <mrow>p(x)q(x)\amp = a_0x^0 \cdot q(x) + a_1x^1 \cdot q(x) + \ldots + a_Nx^N \cdot q(x)</mrow>
      <mrow>\amp = \sum^M_{m=0} a_mx^m \cdot q(x)</mrow>
      <mrow>\amp = \sum^M_{m=0} a_mx^m \cdot \left(\sum^{N}_{n=0} b_n x^n\right)</mrow>
    </md>,
    where in the last equation we have replaced <m>q(x)</m> with its expression in summation notation.
    Now since <m>a_mx^m</m> is constant with respect to <m>n</m>,
    we may pull <m>a_mx^m</m> inside the sum over <m>n</m>,
    which gives:
    <me>
      p(x) q(x) =\sum_{m=0}^{M}\sum_{n=0}^{N}(a_mx^m) b_n x^{n}=\sum_{m=0}^{M}\sum_{n=0}^{N}a_m b_n x^{m+n}
    </me>,
    where we have used our multiplication rule for monomials:
    <m>(a_mx^m) b_n x^{n}=a_m b_n x^{m+n}</m>.
  </p>
  <p>
    Although this expression is correct,
    it's kind of a hodgepodge.
    The reason is that not all the terms with the same power of <m>x</m> are grouped together.
    So let's try to collect terms according to like power of <m>x</m>.
  </p>
  <p>
    We'll start with <m>x^0</m>.
    Since terms have the form <m>a_m b_n x^{m+n}</m>,
    this means we need to find all values of <m>m</m> and <m>n</m> such that <m>m+n=0</m>.
    Since both <m>m</m> and <m>n</m> are nonnegative,
    the only possibility is <m>m=0,n=0</m>,
    which gives the term <m>a_0 b_0 x^{0}</m>.
  </p>
  <p>
    Next let's look at <m>x^1</m>.
    In this case we want terms
    <m>a_m b_n x^{m+n}</m> which have <m>m+n=1</m>.
    There are two: <m>a_1 b_0 x^{1}</m> and <m>a_0 b_1 x^{1}</m>.
  </p>
  <p>
    If we treat <m>x^2</m> similarly, we have three terms:
    <m>a_2 b_0 x^{2}</m>, <m>a_1 b_1 x^{2}</m>, and <m>a_0 b_2 x^{2}</m>.
    Then <m>x^3</m> has four terms:
    <m>a_3 b_0 x^{3}</m>, <m>a_2 b_1 x^{3}</m>,
    <m>a_1b_2 x^{3}</m>, and <m>a_0b_3x^3</m>.
    Do you see the pattern?
    For <m>x^k</m> we will get <m>k+1</m> terms:
    <m>a_k b_0 x^{k}</m>, <m>a_{k-1} b_1 x^{k}</m>, <m>\ldots</m>,
    <m>a_1 b_{k-1} x^{k}</m>, and <m>a_0 b_{k} x^{k}</m>.
    Since <m>+</m> is commutative,
    we may sum these terms together to obtain the coefficient of <m>x^k</m>,
    which we will denote as <m>c_k</m>:
    <me>
      c_k  = a_0  b_k + a_1 b_{k -1} + \cdots + a_{k -1} b _1 + a_k b_0 = \sum_{j = 0}^k a_j b_{k - j}
    </me>,
  </p>
  <p>
    This is the coefficient of <m>x^k</m> in the summation notation expression for the product.
    At last we have our general formula:
  </p>
  <definition>
    <statement>
      <p>
        {defprodpoly} The <em>product of two polynomials</em><idx><h>Product</h><h>of polynomials</h></idx>
            <idx><h>Polynomials</h><h>product</h></idx> <m>p(x)= \sum^{M}_{m=0} a_m x^m</m> and <m>q(x)=\sum^{N}_{n=0} b_n x^n</m> is given by:
        <me>
          p(x) q(x) = \sum_{k=0}^{M+N} c_k x^k
        </me>,
        where
        <me>
          c_k=  \sum_{j = 0}^k a_j b_{k - j}
        </me>
        for each <m>k</m>.
      </p>
    </statement>
  </definition>
  <p>
    Let's verify the formula by computing <m>f(x)</m>, where:
    <me>
      f(x)=(1+x^2-2x^3)(x+4x^3)
    </me>.
  </p>
  <p>
    <m>f(x)</m> is the product of <m>p(x)</m> and <m>q(x)</m>, where:
    <me>
      p(x)= 1x^0 + 0x^1 + 1x^2 + (-2)x^3   \text{ and }   q(x)= 0x^0 + 1x^1 + 0x^2 + 4x^3
    </me>
  </p>
  <p>
    Both polynomials have degree 3, so the degree of the product is 3+3=6:
    <me>
      p(x) q(x) = \sum_{k=0}^{m+n} c_k  x^k =  \sum_{k=0}^{6} c_k x^k
    </me>.
  </p>
  <p>
    Now all we have to do is find the values of the seven coefficients <m>c_0, \ldots,c_6</m>,
    some of which may be zero.
    Let us start with <m>c_0</m>:
    <me>
      c_0 = \sum_{i = 0}^0 a_i b_{0 - i} = a_0b_0= 0 \cdot 1 = 0
    </me>.
  </p>
  <p>
    Already we've found a term that is zero.
    We still need to find six more coefficients<ndash/>how about we look at the fifth coefficient:
    <me>
      c_4 =  \sum_{i = 0}^4 a_i b_{4 - i} =   a_0b_4 + a_1b_3 +a_2b_2 + a_3b_1 + a_4b_0
    </me>.
  </p>
  <p>
    Notice that <m>a_4=b_4=0</m> since <m>p(x)</m> and <m>q(x)</m> both have degree 3, so the first and last terms are both 0.
    Altogether we have
    <me>
      c_4=0+0\cdot 4+1\cdot 0+(-2)\cdot 1+0=-2
    </me>.
  </p>
  <p>
    Doing the same for the other coefficients gives us:
    <me>
      f(x)= 0x^0+ 1x^1 + 0x^2 + 5x^3 + (-2)x^4 + 4x^5 + (-8)x^6
    </me>
  </p>
  <p>
    Getting rid of the zero terms and dealing with the negatives gives us the simplified version:
    <me>
      f(x)=x+5x^3-2x^4+4x^5-8x^6
    </me>.
  </p>
  <exercise xml:id="exercise_Polynomials_mult2way">
    <statement>
      <p>
        Perform the following polynomial multiplications in two ways:
        first, by following the procedure described in <xref ref="sec_Polynomials_PolynomialArithmetic">Section</xref>;
        and second, by using the coefficient formula in <xref ref="definition_Polynomials_defprodpoly">Definition</xref> directly.
        Verify that the two methods agree.
        <ol type="a">
          <li>
            <p>
              <m>(-5+x)(3x+ x^2)</m>
            </p>
          </li>
          <li>
            <p>
              <m>(-\sqrt{3}+x)(2\sqrt{3}+5x^3)</m>
            </p>
          </li>
          <li>
            <p>
              <m>(7/2- 3x+4x^2)(2+x^3)</m>
            </p>
          </li>
          <li>
            <p>
              <m>(- 7x^2 + 4x^3+8x^5 )(3-5x+10x^2 )</m>
            </p>
          </li>
        </ol>
      </p>
    </statement>
  </exercise>
  <p>
    The coefficient formula enables us to compute a single coefficient for a product of polynomials without having to compute the rest of the product.
    Here are some exercises for practice:
  </p>
  <exercise xml:id="exercise_Polynomials_multform">
    <statement>
      <ol type="a">
        <li>
          <p>
            Give the coefficient of <m>x^{100}</m> in the polynomial <m>p(x)^2</m>,
            where <m>p(x) = \sum_{n=0}^{100} x^n</m>.
          </p>
        </li>
        <li>
          <p>
            Give the coefficient of <m>x^{25}</m> in the polynomial <m>p(x) \cdot q(x)</m>,
            where <m>p(x) = \sum_{n=0}^{25} nx^n</m> and <m>q(x) = \sum_{m=0}^{25} x^m</m>.
          </p>
        </li>
        <li>
          <p>
            give the coefficient of <m>x^{33}</m> in the polynomial <m>p(x) \cdot q(x)</m>,
            where <m>p(x) = \sum_{n=1}^{33} \frac{x^n}{n}</m> and <m>q(x) = \sum_{n=0}^{32} (33-n)x^n</m>.
          </p>
        </li>
      </ol>
    </statement>
  </exercise>
</section>