<section xml:id="sec_Polynomials_PolynomialArithmetic">
  <title>Review of polynomial arithmetic<nbsp/><nbsp/></title>
  <figure>
    <video youtubeplaylist="PL2uooHqQ6T7PW5na4EX8rQX2WvBBdM8Qo"/>
  </figure>
  <p>
    Let's briefly review what you've previously learned about polynomial arithmetic in earlier algebra classes.
    In this section we'll cover polynomial addition,
    subtraction, and multiplication.
    Polynomial division is a bit more complicated,
    so we'll talk about that later.
  </p>
  <p>
    In your earlier classes,
    most likely you considered polynomials with integer,
    rational, or real coefficients.
    But everything we do in this chapter also applies to polynomials with complex coefficients.
    And in fact,
    there are even more exotic types of polynomials to which the same formulas and results apply.
    We'll consider these later in the chapter.
  </p>
  <p>
    We'll begin with an example.
    Let
    <me>
      p(x)  = x^3 -3x +2   \text{ and }   q(x)  = 5x^3+3x^2 -6x +5
    </me>.
  </p>
  <p>
    Then we can add <m>p(x)</m> and <m>q(x)</m> as follows:
    <md>
      <mrow>p(x) + q(x) \amp  =  ( x^3 - 3 x + 2 ) + ( 5x^3+3 x^2 - 6 x + 5 )</mrow>
      <mrow>\amp  =   (1+5)x^3 +3x^2+(-3-6)x + (2+5)</mrow>
      <mrow>\amp  = 6x^3 + 3 x^2 - 9 x + 7</mrow>
    </md>
  </p>
  <p>
    Notice, we first grouped together terms with the same power of <m>x</m>,
    and then we added the coefficients.
  </p>
  <p>
    Multiplication of polynomials is a bit more involved,
    so we'll start with polynomials of single terms (monomials) and work our way up from there.
    Suppose we have:
    <md>
      <mrow>p(x)  = 5x^3\text{ and } q(x)  = 3x^2</mrow>
    </md>.
  </p>
  <p>
    Then their product is
    <md>
      <mrow>p(x)  q(x) \amp  =  5x^3 3 x^2</mrow>
      <mrow>\amp  = (5 \cdot 3)x^{(3 + 2)},</mrow>
      <mrow>\amp  = 15x^5</mrow>
    </md>,
    where we combined the coefficients and the exponents
    (remember your exponent rules!).
  </p>
  <p>
    Let's extend ourselves a bit and multiply a polynomial of two terms by a monomial:
    <md>
      <mrow>p(x)  = 5x^3 + 2x \text{ and } q(x)  = 3x^2</mrow>
    </md>.
  </p>
  <p>
    According to the distributive law,
    we multiply each term in the first polynomial with the second polynomial:
    <md>
      <mrow>p(x)  q(x) \amp  = ( 5x^3 +2x)  3x^2</mrow>
      <mrow>\amp = 5x^3 3x^2 + 2x 3x^2</mrow>
      <mrow>\amp  = (5 \cdot 3)x^{(3 + 2)} + (2 \cdot 3)x^{(1+2)}</mrow>
      <mrow>\amp  = 15x^5 + 6x^3</mrow>
    </md>.
  </p>
  <p>
    In order to multiply a two term polynomial by another two term polynomial, e.g.
    <md>
      <mrow>p(x)  = 5x^3 + 2x \text{ and }  q(x)  = 3x^2 - 6x</mrow>
    </md>,
    we extend the distributive law even further.
    Like before,
    each term in the first polynomial is being multiplied by the second polynomial.
    Then the product is
    <md>
      <mrow>p(x)  q(x) \amp  = ( 5x^3 +2x)  (3x^2 - 6x)</mrow>
      <mrow>\amp  = 5x^3 (3x^2 - 6x) +2x(3x^2 - 6x)</mrow>
    </md>
  </p>
  <p>
    At this point we just have the sum of two terms,
    each involving a monomials times a two-term polynomial,
    which we now know can be calculated using the distributive property,
    <md>
      <mrow>\amp  = 5x^3 (3x^2 - 6x) +2x(3x^2 - 6x)</mrow>
      <mrow>\amp  = (15x^5 -30x^4) + (6x^3-12x^2)</mrow>
      <mrow>\amp = 15x^5 - 30x^4 + 6x^3 - 12x^2</mrow>
    </md>
  </p>
  <p>
    This is just the same result as the FOIL method
        <idx><h>FOIL (FLOI) method</h></idx>
    you learned in high school,
    but thinking in terms of the distributive property has the advantage of being applicable to polynomials that have more than just two terms each.
    For instance, with
    <md>
      <mrow>p(x)  = 5x^3 + 4x^2 - 2x \text{ and }  q(x)  = 3x^2 - 6x</mrow>
    </md>,
    we obtain
    <md>
      <mrow>p(x) q(x) \amp  = 5x^3 (3x^2 - 6x) +4x^2(3x^2 - 6x)-2x(3x^2 - 6x)</mrow>
      <mrow>\amp  = (15x^5 -30x^4) + (12x^4 - 24x^3)  + (-6x^3 + 12x^2)</mrow>
      <mrow>\amp = 15x^5 - 30x^4 + 12x^4-24x^3 - 6x^3 + 12x^2</mrow>
      <mrow>\amp = 15x^5 + (-30+12)x^4 + (-24-6)x^3 +12x^2</mrow>
      <mrow>\amp = 15x^5 - 18x^4 - 30x^3 +12x^2</mrow>
    </md>.
  </p>
  <p>
    Again notice that we are grouping like terms by exponent.
    Later, when we give a more general way of multiplying polynomials,
    this method of distribution is what you need to have in mind.
  </p>
  <exercise xml:id="exercise_Polynomials_poly2">
    <statement>
      <ol type="a">
        <li>
          <p>
            Let <m>p(x)=4x^2+7x</m> and <m>q(x)=-2x^2-3x+2</m>.
            Using polynomial arithmetic,
            compute both the sum and the product of <m>p(x)</m> and <m>q(x)</m>.
          </p>
        </li>
        <li>
          <p>
            Let <m>p(x)=3x^2+8x-2</m> and <m>q(x)=2x^2-5x+9</m>.
            Using polynomial arithmetic,
            compute both the sum and the product of <m>p(x)</m> and <m>q(x)</m>.
          </p>
        </li>
      </ol>
    </statement>
  </exercise>
</section>